Intermediate commit of axiom refactoring.

Structure/Generic/Axioms.lean
@@ -13,13 +13,12 @@
 
 import Structure.Generic.Notation
 
-import mathlib4_experiments.Data.Notation
 import mathlib4_experiments.Data.Equiv.Basic
 
 
 
 set_option autoBoundImplicitLocal false
-set_option pp.universes true
+--set_option pp.universes true
 
 universes u v w
 
@@ -101,8 +100,8 @@ end Universe
 class HasExternalFunctors (U : Universe.{u}) (V : Universe.{v}) : Type (max u v) where
 (IsFun {α : U} {β : V} : (α → β) → Sort (max u v))
 
-structure BundledFunctor {U : Universe.{u}} {V : Universe.{v}}
-          [h : HasExternalFunctors.{u, v} U V] (α : U) (β : V) : Sort (max 1 u v) where
+structure BundledFunctor {U : Universe.{u}} {V : Universe.{v}} [h : HasExternalFunctors U V]
+                         (α : U) (β : V) : Sort (max 1 u v) where
 (f     : α → β)
 (isFun : h.IsFun f)
 
@@ -118,7 +117,7 @@ namespace BundledFunctor
 
 end BundledFunctor
 
-class HasInternalFunctors (U : Universe.{u}) extends HasExternalFunctors.{u, u} U U : Type u where
+class HasInternalFunctors (U : Universe.{u}) extends HasExternalFunctors U U : Type u where
 (Fun                : U → U → U)
 (funEquiv (α β : U) : ⌈Fun α β⌉ ≃ (α ⟶' β))
 
@@ -146,17 +145,26 @@ namespace HasInternalFunctors
 
   @[simp] theorem fromBundled.coe {α β : U} (F : α ⟶' β) : funCoe (fromBundled F) = F.f :=
   congrArg BundledFunctor.f (toFromBundled F)
-
   @[simp] theorem fromBundled.eff {α β : U} (F : α ⟶' β) (a : α) : (fromBundled F) a = F a :=
   congrFun (fromBundled.coe F) a
 
-  def mkFun {α β : U} {f : α → β} (hf : h.IsFun f) : α ⟶  β := fromBundled (BundledFunctor.mkFun hf)
+  def mkFun {α β : U} {f : α → β} (hf : h.IsFun f) : α ⟶ β := fromBundled (BundledFunctor.mkFun hf)
 
   @[simp] theorem mkFun.eff {α β : U} {f : α → β} (hf : h.IsFun f) (a : α) :
     (mkFun hf) a = f a :=
   fromBundled.eff (BundledFunctor.mkFun hf) a
 
 end HasInternalFunctors
+
+
+
+@[simp] theorem elimRec {α : Sort u} {a a' : α} {ha : a = a'}
+                        {T : α → Sort v} {x : T a}
+                        {β : Sort w} {f : {a : α} → T a → β} :
+  @f a' (ha ▸ x) = f x :=
+by subst ha; rfl
+
+
 
 -- The following axioms are equivalent to asserting the existence of five functors with specified behavior:
 -- id    : `α ⟶ α,                           a ↦ a`
@@ -165,10 +173,10 @@ end HasInternalFunctors
 -- dup   : `(α ⟶ α ⟶ β) ⟶ (α ⟶ β),           F ↦ (a ↦ F a a)`
 -- comp  : `(α ⟶ β) ⟶ (β ⟶ γ) ⟶ (α ⟶ γ),     F ↦ (G ↦ (a ↦ G (F a)))`
 --
--- We construct these functors below. In `DerivedFunctors.lean`, we additionally construct e.g.
+-- From these, we can construct several other functors such as
 -- swap  : `(α ⟶ β ⟶ γ) ⟶ (β ⟶ α ⟶ γ),       F ↦ (b ↦ (a ↦ F a b))`
 -- subst : `(α ⟶ β ⟶ γ) ⟶ (α ⟶ β) ⟶ (α ⟶ γ), F ↦ (G ↦ (a ↦ F a (G a)))`
--- from these axioms, and give a general algorithm for proving that a function is functorial.
+-- Using these, we can give a general algorithm for proving that a function is functorial.
 
 class HasIdFun (U : Universe) [h : HasExternalFunctors U U] where
 (idIsFun (α : U) : h.IsFun (λ a : α => a))
@@ -206,6 +214,8 @@ namespace HasCompFun
 
 end HasCompFun
 
+
+
 class HasLinearFunOp (U : Universe.{u}) [h : HasInternalFunctors U] extends HasIdFun U, HasCompFun U U U where
 (appIsFun        {α : U} (a : α) (β : U)        : h.IsFun (λ F : α ⟶ β     => F a))
 (appFunIsFun     (α β : U)                      : h.IsFun (λ a : α         => HasInternalFunctors.mkFun (appIsFun a β)))
@@ -216,53 +226,100 @@ namespace HasLinearFunOp
 
   variable {U : Universe.{u}} [HasInternalFunctors U] [h : HasLinearFunOp U]
 
-  def idFun  (α : U) : α ⟶  α := HasInternalFunctors.mkFun (h.idIsFun α)
   def idFun' (α : U) : α ⟶' α := HasIdFun.idFun' α
+  def idFun  (α : U) : α ⟶  α := HasInternalFunctors.fromBundled (idFun' α)
 
   @[simp] theorem idFun.eff (α : U) (a : α) : (idFun α) a = a :=
-  by apply HasInternalFunctors.mkFun.eff
+  by apply HasInternalFunctors.fromBundled.eff
 
-  def appFun' {α : U} (a : α) (β : U) : (α ⟶ β) ⟶' β := BundledFunctor.mkFun      (h.appIsFun a β)
-  def appFun  {α : U} (a : α) (β : U) : (α ⟶ β) ⟶  β := HasInternalFunctors.mkFun (h.appIsFun a β)
+  def appFun' {α : U} (a : α) (β : U) : (α ⟶ β) ⟶' β := BundledFunctor.mkFun (h.appIsFun a β)
+  def appFun  {α : U} (a : α) (β : U) : (α ⟶ β) ⟶  β := HasInternalFunctors.fromBundled (appFun' a β)
 
   @[simp] theorem appFun.eff {α : U} (a : α) (β : U) (F : α ⟶ β) : (appFun a β) F = F a :=
-  by apply HasInternalFunctors.mkFun.eff
+  by apply HasInternalFunctors.fromBundled.eff
 
-  def appFunFun' (α β : U) : α ⟶' (α ⟶ β) ⟶ β := BundledFunctor.mkFun      (h.appFunIsFun α β)
-  def appFunFun  (α β : U) : α ⟶  (α ⟶ β) ⟶ β := HasInternalFunctors.mkFun (h.appFunIsFun α β)
+  def appFunFun' (α β : U) : α ⟶' (α ⟶ β) ⟶ β := BundledFunctor.mkFun (h.appFunIsFun α β)
+  def appFunFun  (α β : U) : α ⟶  (α ⟶ β) ⟶ β := HasInternalFunctors.fromBundled (appFunFun' α β)
 
   @[simp] theorem appFunFun.eff (α β : U) (a : α) : (appFunFun α β) a = appFun a β :=
-  by apply HasInternalFunctors.mkFun.eff
-
+  by apply HasInternalFunctors.fromBundled.eff
   @[simp] theorem appFunFun.effEff (α β : U) (a : α) (F : α ⟶ β) : ((appFunFun α β) a) F = F a :=
   by simp
 
   def compFun' {α β γ : U} (F : α ⟶' β) (G : β ⟶' γ) : α ⟶' γ := HasCompFun.compFun' F G
-  def compFun  {α β γ : U} (F : α ⟶  β) (G : β ⟶  γ) : α ⟶  γ := HasInternalFunctors.mkFun (h.compIsFun (HasInternalFunctors.toBundled F) (HasInternalFunctors.toBundled G))
+  def compFun  {α β γ : U} (F : α ⟶  β) (G : β ⟶  γ) : α ⟶  γ :=
+  HasInternalFunctors.fromBundled (compFun' (HasInternalFunctors.toBundled F) (HasInternalFunctors.toBundled G))
 
   @[simp] theorem compFun.eff {α β γ : U} (F : α ⟶ β) (G : β ⟶ γ) (a : α) : (compFun F G) a = G (F a) :=
-  by apply HasInternalFunctors.mkFun.eff
+  by apply HasInternalFunctors.fromBundled.eff
 
-  def compFunFun' {α β : U} (F : α ⟶' β) (γ : U) : (β ⟶ γ) ⟶' (α ⟶ γ) := BundledFunctor.mkFun      (h.compFunIsFun F                                 γ)
-  def compFunFun  {α β : U} (F : α ⟶  β) (γ : U) : (β ⟶ γ) ⟶  (α ⟶ γ) := HasInternalFunctors.mkFun (h.compFunIsFun (HasInternalFunctors.toBundled F) γ)
+  def compFunFun' {α β : U} (F : α ⟶' β) (γ : U) : (β ⟶ γ) ⟶' (α ⟶ γ) := BundledFunctor.mkFun (h.compFunIsFun F γ)
+  def compFunFun  {α β : U} (F : α ⟶  β) (γ : U) : (β ⟶ γ) ⟶  (α ⟶ γ) :=
+  HasInternalFunctors.fromBundled (compFunFun' (HasInternalFunctors.toBundled F) γ)
 
   @[simp] theorem compFunFun.eff {α β : U} (F : α ⟶ β) (γ : U) (G : β ⟶ γ) : (compFunFun F γ) G = compFun F G :=
-  by apply HasInternalFunctors.mkFun.eff
-
+  by apply HasInternalFunctors.fromBundled.eff
   @[simp] theorem compFunFun.effEff {α β : U} (F : α ⟶ β) (γ : U) (G : β ⟶ γ) (a : α) : ((compFunFun F γ) G) a = G (F a) :=
   by simp
 
-  def compFunFunFun' (α β γ : U) : (α ⟶ β) ⟶' (β ⟶ γ) ⟶ (α ⟶ γ) := BundledFunctor.mkFun      (h.compFunFunIsFun α β γ)
-  def compFunFunFun  (α β γ : U) : (α ⟶ β) ⟶  (β ⟶ γ) ⟶ (α ⟶ γ) := HasInternalFunctors.mkFun (h.compFunFunIsFun α β γ)
+  def compFunFunFun' (α β γ : U) : (α ⟶ β) ⟶' (β ⟶ γ) ⟶ (α ⟶ γ) := BundledFunctor.mkFun (h.compFunFunIsFun α β γ)
+  def compFunFunFun  (α β γ : U) : (α ⟶ β) ⟶  (β ⟶ γ) ⟶ (α ⟶ γ) := HasInternalFunctors.fromBundled (compFunFunFun' α β γ)
   
   @[simp] theorem compFunFunFun.eff (α β γ : U) (F : α ⟶ β) : (compFunFunFun α β γ) F = compFunFun F γ :=
-  by apply HasInternalFunctors.mkFun.eff
-
+  by apply HasInternalFunctors.fromBundled.eff
   @[simp] theorem compFunFunFun.effEff (α β γ : U) (F : α ⟶ β) (G : β ⟶ γ) : ((compFunFunFun α β γ) F) G = compFun F G :=
   by simp
-
   @[simp] theorem compFunFunFun.effEffEff (α β γ : U) (F : α ⟶ β) (G : β ⟶ γ) (a : α) : (((compFunFunFun α β γ) F) G) a = G (F a) :=
   by simp
+
+  -- The "swap" functor swaps the arguments of a nested functor. Its plain version `swapFun` actually
+  -- just fixes the second argument.
+
+  def swapIsFun {α β γ : U} (F : α ⟶' β ⟶ γ) (b : β) : HasExternalFunctors.IsFun (λ a : α => F a b) :=
+  h.compIsFun F (appFun' b γ)
+
+  def swapFun' {α β γ : U} (F : α ⟶' β ⟶ γ) (b : β) : α ⟶' γ := BundledFunctor.mkFun (swapIsFun F b)
+  def swapFun  {α β γ : U} (F : α ⟶  β ⟶ γ) (b : β) : α ⟶  γ := HasInternalFunctors.fromBundled (swapFun' (HasInternalFunctors.toBundled F) b)
+
+  @[simp] theorem swapFun.eff {α β γ : U} (F : α ⟶ β ⟶ γ) (b : β) (a : α) : (swapFun F b) a = F a b :=
+  by apply HasInternalFunctors.fromBundled.eff
+
+  theorem swapFunFun.def {α β γ : U} (F : α ⟶' β ⟶ γ) (b : β) :
+    HasInternalFunctors.fromBundled (swapFun' F b) = HasInternalFunctors.fromBundled (HasInternalFunctors.toBundled (appFun b γ) ⊙' F) :=
+  HasInternalFunctors.toFromBundled (appFun' b γ) ▸ rfl
+
+  def swapFunIsFun {α β γ : U} (F : α ⟶' β ⟶ γ) : HasExternalFunctors.IsFun (λ b : β => HasInternalFunctors.fromBundled (swapFun' F b)) :=
+  funext (swapFunFun.def F) ▸ h.compIsFun (appFunFun' β γ) (compFunFun' F γ)
+
+  def swapFunFun' {α β γ : U} (F : α ⟶' β ⟶ γ) : β ⟶' α ⟶ γ := BundledFunctor.mkFun (swapFunIsFun F)
+  def swapFunFun  {α β γ : U} (F : α ⟶  β ⟶ γ) : β ⟶  α ⟶ γ := HasInternalFunctors.fromBundled (swapFunFun' (HasInternalFunctors.toBundled F))
+
+  @[simp] theorem swapFunFun.eff {α β γ : U} (F : α ⟶ β ⟶ γ) (b : β) : (swapFunFun F) b = swapFun F b :=
+  by apply HasInternalFunctors.fromBundled.eff
+
+  @[simp] theorem swapFunFun.effEff {α β γ : U} (F : α ⟶ β ⟶ γ) (b : β) (a : α) : ((swapFunFun F) b) a = F a b :=
+  by simp
+
+  theorem swapFunFunFun.def (α β γ : U) (F : α ⟶ β ⟶ γ) :
+    HasInternalFunctors.mkFun (swapFunIsFun (HasInternalFunctors.toBundled F)) = HasInternalFunctors.fromBundled (HasInternalFunctors.toBundled (compFunFun F γ) ⊙' appFunFun' β γ) :=
+  HasInternalFunctors.toFromBundled (compFunFun' (HasInternalFunctors.toBundled F) γ) ▸ elimRec
+
+  def swapFunFunIsFun (α β γ : U) : HasExternalFunctors.IsFun (λ F : α ⟶ β ⟶ γ => swapFunFun F) :=
+  funext (swapFunFunFun.def α β γ) ▸ h.compIsFun (compFunFunFun' α (β ⟶ γ) γ) (compFunFun' (appFunFun' β γ) (α ⟶ γ))
+
+  def swapFunFunFun' (α β γ : U) : (α ⟶ β ⟶ γ) ⟶' (β ⟶ α ⟶ γ) := BundledFunctor.mkFun (swapFunFunIsFun α β γ)
+  def swapFunFunFun  (α β γ : U) : (α ⟶ β ⟶ γ) ⟶  (β ⟶ α ⟶ γ) := HasInternalFunctors.fromBundled (swapFunFunFun' α β γ)
+
+  @[simp] theorem swapFunFunFun.eff (α β γ : U) (F : α ⟶ β ⟶ γ) : (swapFunFunFun α β γ) F = swapFunFun F :=
+  by apply HasInternalFunctors.fromBundled.eff
+
+  @[simp] theorem swapFunFunFun.effEff (α β γ : U) (F : α ⟶ β ⟶ γ) (b : β) : ((swapFunFunFun α β γ) F) b = swapFun F b :=
+  by simp
+
+  @[simp] theorem swapFunFunFun.effEffEff (α β γ : U) (F : α ⟶ β ⟶ γ) (b : β) (a : α) : (((swapFunFunFun α β γ) F) b) a = F a b :=
+  by simp
+
+  -- In particular, reverse composition is also functorial.
 
   def revCompFun {α β γ : U} (G : β ⟶  γ) (F : α ⟶  β) : α ⟶ γ := compFun F G
   infixr:90 " ⊙ "  => HasLinearFunOp.revCompFun
@@ -270,64 +327,511 @@ namespace HasLinearFunOp
   @[simp] theorem revCompFun.eff {α β γ : U} (F : α ⟶ β) (G : β ⟶ γ) (a : α) : (G ⊙ F) a = G (F a) :=
   compFun.eff F G a
 
+  theorem revCompFunFun.def (α : U) {β γ : U} (G : β ⟶' γ) (F : α ⟶ β) :
+    HasInternalFunctors.fromBundled (G ⊙' HasInternalFunctors.toBundled F) = (compFunFun F γ) (HasInternalFunctors.fromBundled G) :=
+  Eq.subst (motive := λ H => HasInternalFunctors.fromBundled (H ⊙' HasInternalFunctors.toBundled F) = (compFunFun F γ) (HasInternalFunctors.fromBundled G))
+           (HasInternalFunctors.toFromBundled G)
+           (Eq.symm (compFunFun.eff F γ (HasInternalFunctors.fromBundled G)))
+
+  def revCompFunIsFun (α : U) {β γ : U} (G : β ⟶' γ) :
+    HasExternalFunctors.IsFun (λ F : α ⟶ β => HasInternalFunctors.fromBundled (G ⊙' HasInternalFunctors.toBundled F)) :=
+  funext (revCompFunFun.def α G) ▸ swapIsFun (compFunFunFun' α β γ) (HasInternalFunctors.fromBundled G)
+
+  def revCompFunFun' (α : U) {β γ : U} (G : β ⟶' γ) : (α ⟶ β) ⟶' (α ⟶ γ) := BundledFunctor.mkFun (revCompFunIsFun α G)
+  def revCompFunFun  (α : U) {β γ : U} (G : β ⟶  γ) : (α ⟶ β) ⟶  (α ⟶ γ) := HasInternalFunctors.fromBundled (revCompFunFun' α (HasInternalFunctors.toBundled G))
+
+  @[simp] theorem revCompFunFun.eff (α : U) {β γ : U} (G : β ⟶ γ) (F : α ⟶ β) : (revCompFunFun α G) F = G ⊙ F :=
+  by apply HasInternalFunctors.fromBundled.eff
+
+  @[simp] theorem revCompFunFun.effEff (α : U) {β γ : U} (G : β ⟶ γ) (F : α ⟶ β) (a : α) : ((revCompFunFun α G) F) a = G (F a) :=
+  by simp
+
+  theorem revCompFunFunFun.def (α β γ : U) (G : β ⟶ γ) :
+    HasInternalFunctors.mkFun (revCompFunIsFun α (HasInternalFunctors.toBundled G)) = HasInternalFunctors.fromBundled (swapFun' (compFunFunFun' α β γ) G) :=
+  congrArg (λ H => HasInternalFunctors.fromBundled (swapFun' (compFunFunFun' α β γ) H)) (HasInternalFunctors.fromToBundled G) ▸ elimRec
+
+  def revCompFunFunIsFun (α β γ : U) : HasExternalFunctors.IsFun (λ G : β ⟶ γ => revCompFunFun α G) :=
+  funext (revCompFunFunFun.def α β γ) ▸ swapFunIsFun (compFunFunFun' α β γ)
+
+  def revCompFunFunFun' (α β γ : U) : (β ⟶ γ) ⟶' (α ⟶ β) ⟶ (α ⟶ γ) := BundledFunctor.mkFun (revCompFunFunIsFun α β γ)
+  def revCompFunFunFun  (α β γ : U) : (β ⟶ γ) ⟶  (α ⟶ β) ⟶ (α ⟶ γ) := HasInternalFunctors.fromBundled (revCompFunFunFun' α β γ)
+
+  @[simp] theorem revCompFunFunFun.eff (α β γ : U) (G : β ⟶ γ) : (revCompFunFunFun α β γ) G = revCompFunFun α G :=
+  by apply HasInternalFunctors.fromBundled.eff
+
+  @[simp] theorem revCompFunFunFun.effEff (α β γ : U) (G : β ⟶ γ) (F : α ⟶ β) : ((revCompFunFunFun α β γ) G) F = G ⊙ F :=
+  by simp
+
+  @[simp] theorem revCompFunFunFun.effEffEff (α β γ : U) (G : β ⟶ γ) (F : α ⟶ β) (a : α) : (((revCompFunFunFun α β γ) G) F) a = G (F a) :=
+  by simp
+
+  -- Composition of a function with two arguments.
+
+  def compFun₂ {α β γ δ : U} (F : α ⟶ β ⟶ γ) (G : γ ⟶ δ) : α ⟶ β ⟶ δ := swapFunFun (revCompFunFun α G ⊙ swapFunFun F)
+
 end HasLinearFunOp
 
-class HasAffineFunOp (U : Universe.{u}) [h : HasInternalFunctors U] extends HasLinearFunOp U, HasConstFun U U where
+
+
+class HasSubLinearFunOp (U : Universe.{u}) [h : HasInternalFunctors U] extends HasConstFun U U where
 (constFunIsFun (α β : U) : h.IsFun (λ c : β => HasInternalFunctors.mkFun (constIsFun α c)))
 
-namespace HasAffineFunOp
+namespace HasSubLinearFunOp
 
-  variable {U : Universe.{u}} [HasInternalFunctors U] [h : HasAffineFunOp U]
+  variable {U : Universe.{u}} [HasInternalFunctors U] [h : HasSubLinearFunOp U]
 
   def constFun' (α : U) {β : U} (c : β) : α ⟶' β := HasConstFun.constFun' α c
-  def constFun  (α : U) {β : U} (c : β) : α ⟶  β := HasInternalFunctors.mkFun (h.constIsFun α c)
+  def constFun  (α : U) {β : U} (c : β) : α ⟶  β := HasInternalFunctors.fromBundled (constFun' α c)
 
   @[simp] theorem constFun.eff (α : U) {β : U} (c : β) (a : α) : (constFun α c) a = c :=
-  by apply HasInternalFunctors.mkFun.eff
+  by apply HasInternalFunctors.fromBundled.eff
 
-  def constFunFun' (α β : U) : β ⟶' (α ⟶ β) := BundledFunctor.mkFun      (h.constFunIsFun α β)
-  def constFunFun  (α β : U) : β ⟶  (α ⟶ β) := HasInternalFunctors.mkFun (h.constFunIsFun α β)
+  def constFunFun' (α β : U) : β ⟶' (α ⟶ β) := BundledFunctor.mkFun (h.constFunIsFun α β)
+  def constFunFun  (α β : U) : β ⟶  (α ⟶ β) := HasInternalFunctors.fromBundled (constFunFun' α β)
 
   @[simp] theorem constFunFun.eff (α β : U) (c : β) : (constFunFun α β) c = constFun α c :=
-  by apply HasInternalFunctors.mkFun.eff
-
+  by apply HasInternalFunctors.fromBundled.eff
   @[simp] theorem constFunFun.effEff (α β : U) (c : β) (a : α) : ((constFunFun α β) c) a = c :=
   by simp
 
-end HasAffineFunOp
+end HasSubLinearFunOp
 
-class HasFullFunOp (U : Universe.{u}) [h : HasInternalFunctors U] extends HasAffineFunOp U where
+class HasAffineFunOp (U : Universe.{u}) [h : HasInternalFunctors U] extends HasLinearFunOp U, HasSubLinearFunOp U
+
+
+
+class HasNonLinearFunOp (U : Universe.{u}) [h : HasInternalFunctors U] where
 (dupIsFun    {α β : U} (F : α ⟶' α ⟶ β) : h.IsFun (λ a : α         => F a a))
 (dupFunIsFun (α β : U)                  : h.IsFun (λ F : α ⟶ α ⟶ β => HasInternalFunctors.mkFun (dupIsFun (HasInternalFunctors.toBundled F))))
+
+namespace HasNonLinearFunOp
+
+  variable {U : Universe.{u}} [HasInternalFunctors U] [h : HasNonLinearFunOp U]
+
+  def dupFun' {α β : U} (F : α ⟶' α ⟶ β) : α ⟶' β := BundledFunctor.mkFun (h.dupIsFun F)
+  def dupFun  {α β : U} (F : α ⟶  α ⟶ β) : α ⟶  β :=
+  HasInternalFunctors.fromBundled (dupFun' (HasInternalFunctors.toBundled F))
+
+  @[simp] theorem dupFun.eff {α β : U} (F : α ⟶ α ⟶ β) (a : α) : (dupFun F) a = F a a :=
+  by apply HasInternalFunctors.fromBundled.eff
+
+  def dupFunFun' (α β : U) : (α ⟶ α ⟶ β) ⟶' (α ⟶ β) := BundledFunctor.mkFun (h.dupFunIsFun α β)
+  def dupFunFun  (α β : U) : (α ⟶ α ⟶ β) ⟶  (α ⟶ β) := HasInternalFunctors.fromBundled (dupFunFun' α β)
+
+  @[simp] theorem dupFunFun.eff (α β : U) (F : α ⟶ α ⟶ β) : (dupFunFun α β) F = dupFun F :=
+  by apply HasInternalFunctors.fromBundled.eff
+  @[simp] theorem dupFunFun.effEff (α β : U) (F : α ⟶ α ⟶ β) (a : α) : ((dupFunFun α β) F) a = F a a :=
+  by simp
+
+end HasNonLinearFunOp
+
+class HasFullFunOp (U : Universe.{u}) [h : HasInternalFunctors U] extends HasAffineFunOp U, HasNonLinearFunOp U
 
 namespace HasFullFunOp
 
   variable {U : Universe.{u}} [HasInternalFunctors U] [h : HasFullFunOp U]
 
-  def dupFun' {α β : U} (F : α ⟶' α ⟶ β) : α ⟶' β := BundledFunctor.mkFun      (h.dupIsFun F)
-  def dupFun  {α β : U} (F : α ⟶  α ⟶ β) : α ⟶  β := HasInternalFunctors.mkFun (h.dupIsFun (HasInternalFunctors.toBundled F))
+  -- The S combinator (see https://en.wikipedia.org/wiki/SKI_combinator_calculus), which in our case says
+  -- that if we can functorially construct a functor `H : β ⟶ γ` and an argument `b : β`, then the
+  -- construction of `H b` is also functorial.
 
-  @[simp] theorem dupFun.eff {α β : U} (F : α ⟶ α ⟶ β) (a : α) : (dupFun F) a = F a a :=
-  by apply HasInternalFunctors.mkFun.eff
+  theorem substFun.def {α β γ : U} (F : α ⟶' β ⟶ γ) (G : α ⟶' β) (a : α) :
+    F a (G a) = HasInternalFunctors.fromBundled (HasLinearFunOp.swapFun' F (G a)) a :=
+  Eq.symm (HasInternalFunctors.fromBundled.eff (HasLinearFunOp.swapFun' F (G a)) a)
 
-  def dupFunFun' (α β : U) : (α ⟶ α ⟶ β) ⟶' (α ⟶ β) := BundledFunctor.mkFun      (h.dupFunIsFun α β)
-  def dupFunFun  (α β : U) : (α ⟶ α ⟶ β) ⟶  (α ⟶ β) := HasInternalFunctors.mkFun (h.dupFunIsFun α β)
+  def substIsFun {α β γ : U} (F : α ⟶' β ⟶ γ) (G : α ⟶' β) : HasExternalFunctors.IsFun (λ a : α => F a (G a)) :=
+  funext (substFun.def F G) ▸ h.dupIsFun (HasLinearFunOp.swapFunFun' F ⊙' G)
 
-  @[simp] theorem dupFunFun.eff (α β : U) (F : α ⟶ α ⟶ β) : (dupFunFun α β) F = dupFun F :=
-  by apply HasInternalFunctors.mkFun.eff
+  def substFun' {α β γ : U} (F : α ⟶' β ⟶ γ) (G : α ⟶' β) : α ⟶' γ := BundledFunctor.mkFun (substIsFun F G)
+  def substFun  {α β γ : U} (F : α ⟶  β ⟶ γ) (G : α ⟶  β) : α ⟶  γ := HasInternalFunctors.fromBundled (substFun' (HasInternalFunctors.toBundled F) (HasInternalFunctors.toBundled G))
 
-  @[simp] theorem dupFunFun.effEff (α β : U) (F : α ⟶ α ⟶ β) (a : α) : ((dupFunFun α β) F) a = F a a :=
+  @[simp] theorem substFun.eff {α β γ : U} (F : α ⟶ β ⟶ γ) (G : α ⟶ β) (a : α) : (substFun F G) a = F a (G a) :=
+  by apply HasInternalFunctors.fromBundled.eff
+
+  theorem substFunFun.def {α β γ : U} (F : α ⟶' β ⟶ γ) (G : α ⟶ β) :
+    HasInternalFunctors.mkFun (substIsFun F (HasInternalFunctors.toBundled G)) =
+    HasInternalFunctors.fromBundled (HasNonLinearFunOp.dupFun' (HasInternalFunctors.toBundled (HasInternalFunctors.fromBundled (HasLinearFunOp.swapFunFun' F ⊙' HasInternalFunctors.toBundled G)))) :=
+  HasInternalFunctors.toFromBundled _ ▸ elimRec
+
+  def substFunIsFun {α β γ : U} (F : α ⟶' β ⟶ γ) :
+    HasExternalFunctors.IsFun (λ G : α ⟶ β => HasInternalFunctors.fromBundled (substFun' F (HasInternalFunctors.toBundled G))) :=
+  funext (substFunFun.def F) ▸ h.compIsFun (HasLinearFunOp.revCompFunFun' α (HasLinearFunOp.swapFunFun' F)) (HasNonLinearFunOp.dupFunFun' α γ)
+
+  def substFunFun' {α β γ : U} (F : α ⟶' β ⟶ γ) : (α ⟶ β) ⟶' (α ⟶ γ) := BundledFunctor.mkFun (substFunIsFun F)
+  def substFunFun  {α β γ : U} (F : α ⟶  β ⟶ γ) : (α ⟶ β) ⟶  (α ⟶ γ) := HasInternalFunctors.fromBundled (substFunFun' (HasInternalFunctors.toBundled F))
+
+  @[simp] theorem substFunFun.eff {α β γ : U} (F : α ⟶ β ⟶ γ) (G : α ⟶ β) : (substFunFun F) G = substFun F G :=
+  by apply HasInternalFunctors.fromBundled.eff
+
+  @[simp] theorem substFunFun.effEff {α β γ : U} (F : α ⟶ β ⟶ γ) (G : α ⟶ β) (a : α) : ((substFunFun F) G) a = F a (G a) :=
+  by simp
+
+  theorem substFunFunFun.def (α β γ : U) (F : α ⟶ β ⟶ γ) :
+    HasInternalFunctors.mkFun (substFunIsFun (HasInternalFunctors.toBundled F)) = HasInternalFunctors.fromBundled (HasNonLinearFunOp.dupFunFun' α γ ⊙' HasInternalFunctors.toBundled (HasLinearFunOp.revCompFunFun α (HasLinearFunOp.swapFunFun F))) :=
+  HasInternalFunctors.toFromBundled _ ▸ HasInternalFunctors.toFromBundled _ ▸ elimRec
+
+  def substFunFunIsFun (α β γ : U) : HasExternalFunctors.IsFun (λ F : α ⟶ β ⟶ γ => substFunFun F) :=
+  funext (substFunFunFun.def α β γ) ▸ h.compIsFun (HasLinearFunOp.revCompFunFunFun' α β (α ⟶ γ) ⊙' HasLinearFunOp.swapFunFunFun' α β γ)
+                                                  (HasLinearFunOp.revCompFunFun' (α ⟶ β) (HasNonLinearFunOp.dupFunFun' α γ))
+
+  def substFunFunFun' (α β γ : U) : (α ⟶ β ⟶ γ) ⟶' (α ⟶ β) ⟶ (α ⟶ γ) := BundledFunctor.mkFun (substFunFunIsFun α β γ)
+  def substFunFunFun  (α β γ : U) : (α ⟶ β ⟶ γ) ⟶  (α ⟶ β) ⟶ (α ⟶ γ) := HasInternalFunctors.fromBundled (substFunFunFun' α β γ)
+
+  @[simp] theorem substFunFunFun.eff (α β γ : U) (F : α ⟶ β ⟶ γ) : (substFunFunFun α β γ) F = substFunFun F :=
+  by apply HasInternalFunctors.fromBundled.eff
+
+  @[simp] theorem substFunFunFun.effEff (α β γ : U) (F : α ⟶ β ⟶ γ) (G : α ⟶ β) : ((substFunFunFun α β γ) F) G = substFun F G :=
+  by simp
+
+  @[simp] theorem substFunFunFun.effEffEff (α β γ : U) (F : α ⟶ β ⟶ γ) (G : α ⟶ β) (a : α) : (((substFunFunFun α β γ) F) G) a = F a (G a) :=
   by simp
 
 end HasFullFunOp
 
-class HasFunOp (U : Universe.{u}) extends HasInternalFunctors.{u} U, HasFullFunOp U : Type u
+
+
+-- Using the functoriality axioms and the constructions above, we can algorithmically prove
+-- functoriality of lambda terms. The algorithm to prove `HasExternalFunctors.IsFun (λ a : α => t)`
+-- is as follows:
+--
+--  Case                           | Proof
+-- --------------------------------+--------------------------------------------------------------
+--  `t` does not contain `a`       | `constIsFun α t`
+--  `t` is `a`                     | `idIsFun α`
+--  `t` is `G b` with `G : β ⟶ γ`: |
+--    `a` appears only in `b`      | Prove that `λ a => b` is functorial, yielding a functor
+--                                 | `F : α ⟶ β`. Then the proof is `compIsFun F G`.
+--      `b` is `a`                 | Optimization: `HasInternalFunctors.isFun G`
+--    `a` appears only in `G`      | Prove that `λ a => G` is functorial, yielding a functor
+--                                 | `F : α ⟶ β ⟶ γ`. Then the proof is `swapIsFun F b`.
+--      `G` is `a`                 | Optimization: `appIsFun b γ`
+--    `a` appears in both          | Prove that `λ a => G` is functorial, yielding a functor
+--                                 | `F₁ : α ⟶ β ⟶ γ`. Prove that `λ a => b` is functorial,
+--                                 | yielding a functor `F₂ : α ⟶ β`. Then the proof is
+--                                 | `substIsFun F₁ F₂`.
+--  `t` is `mkFun (λ b : β => c)`  | Prove that `λ a => c` is functorial when regarding `b` as
+--                                 | a constant, yielding a functor `F : α ⟶ γ` for every `b`.
+--                                 | Prove that  `λ b => F` is functorial, yielding a functor
+--                                 | `G : β ⟶ α ⟶ γ`. Then the proof is `swapFunIsFun G`.
+--
+-- (This list does not contain all possible optimizations.)
 
 
 
--- TODO: Introduce products (with functorial construction and projection)
---       and equivalences (with functorial projection to product of to/inv functors)
--- We should be able to prove the arrow/product laws.
+class HasFunOp (U : Universe.{u}) extends HasInternalFunctors U, HasFullFunOp U : Type u
+
+
+
+class HasExternalEquivalences (U : Universe.{u}) (V : Universe.{v})
+                              [hUV : HasExternalFunctors U V] [hVU : HasExternalFunctors V U] : Type (max u v) where
+(IsEquiv {α : U} {β : V} : (α ⟶' β) → (β ⟶' α) → Sort (max u v))
+
+structure BundledEquivalence {U : Universe.{u}} {V : Universe.{v}}
+                             [hUV : HasExternalFunctors U V] [hVU : HasExternalFunctors V U]
+                             [h : HasExternalEquivalences U V]
+                             (α : U) (β : V) : Sort (max 1 u v) where
+(toFun   : α ⟶' β)
+(invFun  : β ⟶' α)
+(isEquiv : h.IsEquiv toFun invFun)
+
+namespace BundledEquivalence
+
+  infix:20 " ⟷' " => BundledEquivalence
+
+  variable {U V : Universe} [hUV : HasExternalFunctors U V] [hVU : HasExternalFunctors V U]
+           [h : HasExternalEquivalences U V]
+
+  def mkEquiv {α : U} {β : V} {to : α ⟶' β} {inv : β ⟶' α} (he : h.IsEquiv to inv) : α ⟷' β :=
+  ⟨to, inv, he⟩
+
+end BundledEquivalence
+
+class HasInternalEquivalences (U : Universe.{u}) [h : HasInternalFunctors U] extends HasExternalEquivalences U U : Type u where
+(Equiv                          : U → U → U)
+(equivEquiv           (α β : U) : ⌈Equiv α β⌉ ≃ (α ⟷' β))
+(equivElimToFunIsFun  (α β : U) : h.IsFun (λ E : Equiv α β => HasInternalFunctors.fromBundled ((equivEquiv α β).toFun E).toFun))
+(equivElimInvFunIsFun (α β : U) : h.IsFun (λ E : Equiv α β => HasInternalFunctors.fromBundled ((equivEquiv α β).toFun E).invFun))
+
+namespace HasInternalEquivalences
+
+  infix:20 " ⟷ " => HasInternalEquivalences.Equiv
+
+  variable {U : Universe} [HasInternalFunctors U] [h : HasInternalEquivalences U]
+
+  def toBundled   {α β : U} (E : α ⟷  β) : α ⟷' β := (h.equivEquiv α β).toFun  E
+  def fromBundled {α β : U} (E : α ⟷' β) : α ⟷  β := (h.equivEquiv α β).invFun E
+
+  @[simp] theorem fromToBundled {α β : U} (E : α ⟷  β) : fromBundled (toBundled E) = E :=
+  (h.equivEquiv α β).leftInv  E
+  @[simp] theorem toFromBundled {α β : U} (E : α ⟷' β) : toBundled (fromBundled E) = E :=
+  (h.equivEquiv α β).rightInv E
+
+  def to  {α β : U} (E : α ⟷ β) (a : α) : β := (toBundled E).toFun  a
+  def inv {α β : U} (E : α ⟷ β) (b : β) : α := (toBundled E).invFun b
+
+  def toFun  {α β : U} (E : α ⟷ β) : α ⟶ β := HasInternalFunctors.fromBundled (toBundled E).toFun
+  def invFun {α β : U} (E : α ⟷ β) : β ⟶ α := HasInternalFunctors.fromBundled (toBundled E).invFun
+
+  @[simp] theorem toFun.eff  {α β : U} (E : α ⟷ β) (a : α) : (toFun  E) a = to  E a :=
+  by apply HasInternalFunctors.fromBundled.eff
+  @[simp] theorem invFun.eff {α β : U} (E : α ⟷ β) (b : β) : (invFun E) b = inv E b :=
+  by apply HasInternalFunctors.fromBundled.eff
+
+  def toFunFun'  (α β : U) : (α ⟷ β) ⟶' (α ⟶ β) := BundledFunctor.mkFun (h.equivElimToFunIsFun  α β)
+  def invFunFun' (α β : U) : (α ⟷ β) ⟶' (β ⟶ α) := BundledFunctor.mkFun (h.equivElimInvFunIsFun α β)
+  def toFunFun   (α β : U) : (α ⟷ β) ⟶  (α ⟶ β) := HasInternalFunctors.fromBundled (toFunFun'  α β)
+  def invFunFun  (α β : U) : (α ⟷ β) ⟶  (β ⟶ α) := HasInternalFunctors.fromBundled (invFunFun' α β)
+
+  @[simp] theorem toFunFun.eff  {α β : U} (E : α ⟷ β) : (toFunFun  α β) E = toFun  E :=
+  by apply HasInternalFunctors.fromBundled.eff
+  @[simp] theorem invFunFun.eff {α β : U} (E : α ⟷ β) : (invFunFun α β) E = invFun E :=
+  by apply HasInternalFunctors.fromBundled.eff
+  @[simp] theorem toFunFun.effEff  {α β : U} (E : α ⟷ β) (a : α) : ((toFunFun  α β) E) a = to  E a :=
+  by simp
+  @[simp] theorem invFunFun.effEff {α β : U} (E : α ⟷ β) (b : β) : ((invFunFun α β) E) b = inv E b :=
+  by simp
+
+  @[simp] theorem toFun.bundledEq  {α β : U} (E : α ⟷ β) : HasInternalFunctors.toBundled (toFun E)  = (toBundled E).toFun :=
+  HasInternalFunctors.toFromBundled (toBundled E).toFun
+  @[simp] theorem invFun.bundledEq {α β : U} (E : α ⟷ β) : HasInternalFunctors.toBundled (invFun E) = (toBundled E).invFun :=
+  HasInternalFunctors.toFromBundled (toBundled E).invFun
+
+  def isEquiv {α β : U} (E : α ⟷ β) : h.IsEquiv (toBundled E).toFun (toBundled E).invFun :=
+  (toBundled E).isEquiv
+
+  def isEquiv' {α β : U} (E : α ⟷ β) :
+    h.IsEquiv (HasInternalFunctors.toBundled (toFun E)) (HasInternalFunctors.toBundled (invFun E)) :=
+  by simp; apply isEquiv
+
+  @[simp] theorem fromBundled.to.coe'  {α β : U} (E : α ⟷' β) : (toBundled (fromBundled E)).toFun  = E.toFun  :=
+  congrArg BundledEquivalence.toFun  (toFromBundled E)
+  @[simp] theorem fromBundled.inv.coe' {α β : U} (E : α ⟷' β) : (toBundled (fromBundled E)).invFun = E.invFun :=
+  congrArg BundledEquivalence.invFun (toFromBundled E)
+  @[simp] theorem fromBundled.to.coe  {α β : U} (E : α ⟷' β) : (toBundled (fromBundled E)).toFun.f  = E.toFun.f  :=
+  congrArg BundledFunctor.f (fromBundled.to.coe'  E)
+  @[simp] theorem fromBundled.inv.coe {α β : U} (E : α ⟷' β) : (toBundled (fromBundled E)).invFun.f = E.invFun.f :=
+  congrArg BundledFunctor.f (fromBundled.inv.coe' E)
+  @[simp] theorem fromBundled.to.eff  {α β : U} (E : α ⟷' β) (a : α) : to  (fromBundled E) a = E.toFun  a :=
+  congrFun (fromBundled.to.coe  E) a
+  @[simp] theorem fromBundled.inv.eff {α β : U} (E : α ⟷' β) (b : β) : inv (fromBundled E) b = E.invFun b :=
+  congrFun (fromBundled.inv.coe E) b
+
+  def mkEquiv {α β : U} {to : α ⟶' β} {inv : β ⟶' α} (he : h.IsEquiv to inv) : α ⟷ β :=
+  fromBundled (BundledEquivalence.mkEquiv he)
+
+end HasInternalEquivalences
+
+class HasIdEquiv (U : Universe) [HasExternalFunctors U U] [HasIdFun U] [h : HasExternalEquivalences U U] where
+(idIsEquiv (α : U) : h.IsEquiv (HasIdFun.idFun' α) (HasIdFun.idFun' α))
+
+namespace HasIdEquiv
+
+  variable {U : Universe} [HasExternalFunctors U U] [HasIdFun U] [HasExternalEquivalences U U] [h : HasIdEquiv U]
+
+  def idEquiv' (α : U) : α ⟷' α := BundledEquivalence.mkEquiv (h.idIsEquiv α)
+
+end HasIdEquiv
+
+class HasCompEquiv (U V W : Universe)
+                   [HasExternalFunctors U V] [HasExternalFunctors V W] [HasExternalFunctors U W]
+                   [HasExternalFunctors V U] [HasExternalFunctors W V] [HasExternalFunctors W U]
+                   [HasCompFun U V W] [HasCompFun W V U]
+                   [HasExternalEquivalences U V] [HasExternalEquivalences V W] [h : HasExternalEquivalences U W] where
+(compIsEquiv {α : U} {β : V} {γ : W} (E : α ⟷' β) (F : β ⟷' γ) : h.IsEquiv (F.toFun ⊙' E.toFun) (E.invFun ⊙' F.invFun))
+
+namespace HasCompEquiv
+
+  variable {U V W : Universe} [HasExternalFunctors U V] [HasExternalFunctors V W] [HasExternalFunctors U W]
+           [HasExternalFunctors V U] [HasExternalFunctors W V] [HasExternalFunctors W U]
+           [HasCompFun U V W] [HasCompFun W V U]
+           [HasExternalEquivalences U V] [HasExternalEquivalences V W] [HasExternalEquivalences U W]
+           [h : HasCompEquiv U V W]
+
+  def compEquiv' {α : U} {β : V} {γ : W} (E : α ⟷' β) (F : β ⟷' γ) : α ⟷' γ := BundledEquivalence.mkEquiv (h.compIsEquiv E F)
+
+end HasCompEquiv
+
+class HasInvEquiv (U V : Universe) [HasExternalFunctors U V] [HasExternalFunctors V U]
+                  [HasExternalEquivalences U V] [h : HasExternalEquivalences V U] where
+(invIsEquiv {α : U} {β : V} (E : α ⟷' β) : h.IsEquiv E.invFun E.toFun)
+
+namespace HasInvEquiv
+
+  variable {U V : Universe} [HasExternalFunctors U V] [HasExternalFunctors V U]
+           [HasExternalEquivalences U V] [HasExternalEquivalences V U] [h : HasInvEquiv U V]
+
+  def invEquiv' {α : U} {β : V} (E : α ⟷' β) : β ⟷' α := BundledEquivalence.mkEquiv (h.invIsEquiv E)
+
+end HasInvEquiv
+
+class HasEquivOp (U : Universe.{u}) [h : HasInternalFunctors U] [HasLinearFunOp U] extends
+  HasInternalEquivalences U, HasIdEquiv U, HasCompEquiv U U U, HasInvEquiv U U : Type u where
+(compEquivIsFun    {α β : U} (E : α ⟷' β) (γ : U) : h.IsFun (λ F : β ⟷ γ => HasInternalEquivalences.mkEquiv (compIsEquiv E (HasInternalEquivalences.toBundled F))))
+(compEquivFunIsFun (α β γ : U)                    : h.IsFun (λ E : α ⟷ β => HasInternalFunctors.mkFun (compEquivIsFun (HasInternalEquivalences.toBundled E) γ)))
+(invEquivIsFun     (α β : U)                      : h.IsFun (λ E : α ⟷ β => HasInternalEquivalences.mkEquiv (invIsEquiv (HasInternalEquivalences.toBundled E))))
+(invEquivIsEquiv   (α β : U)                      : IsEquiv (BundledFunctor.mkFun (invEquivIsFun α β)) (BundledFunctor.mkFun (invEquivIsFun β α)))
+
+namespace HasEquivOp
+
+  variable {U : Universe.{u}} [HasInternalFunctors U] [HasLinearFunOp U] [h : HasEquivOp U]
+
+  def idEquiv' (α : U) : α ⟷' α := HasIdEquiv.idEquiv' α
+  def idEquiv  (α : U) : α ⟷  α := HasInternalEquivalences.fromBundled (idEquiv' α)
+
+  @[simp] theorem idEquiv.to.eff  (α : U) (a : α) : HasInternalEquivalences.to  (idEquiv α) a = a :=
+  by apply HasInternalEquivalences.fromBundled.to.eff
+  @[simp] theorem idEquiv.inv.eff (α : U) (a : α) : HasInternalEquivalences.inv (idEquiv α) a = a :=
+  by apply HasInternalEquivalences.fromBundled.inv.eff
+
+  def compEquiv' {α β γ : U} (E : α ⟷' β) (F : β ⟷' γ) : α ⟷' γ := HasCompEquiv.compEquiv' E F
+  def compEquiv  {α β γ : U} (E : α ⟷  β) (F : β ⟷  γ) : α ⟷  γ :=
+  HasInternalEquivalences.fromBundled (compEquiv' (HasInternalEquivalences.toBundled E) (HasInternalEquivalences.toBundled F))
+
+  @[simp] theorem compEquiv.to.eff  {α β γ : U} (E : α ⟷ β) (F : β ⟷ γ) (a : α) :
+    HasInternalEquivalences.to  (compEquiv E F) a = HasInternalEquivalences.to  F (HasInternalEquivalences.to  E a) :=
+  by apply HasInternalEquivalences.fromBundled.to.eff
+  @[simp] theorem compEquiv.inv.eff {α β γ : U} (E : α ⟷ β) (F : β ⟷ γ) (c : γ) :
+    HasInternalEquivalences.inv (compEquiv E F) c = HasInternalEquivalences.inv E (HasInternalEquivalences.inv F c) :=
+  by apply HasInternalEquivalences.fromBundled.inv.eff
+
+  def compEquivFun' {α β : U} (E : α ⟷' β) (γ : U) : (β ⟷ γ) ⟶' (α ⟷ γ) := BundledFunctor.mkFun (h.compEquivIsFun E γ)
+  def compEquivFun  {α β : U} (E : α ⟷  β) (γ : U) : (β ⟷ γ) ⟶  (α ⟷ γ) :=
+  HasInternalFunctors.fromBundled (compEquivFun' (HasInternalEquivalences.toBundled E) γ)
+
+  @[simp] theorem compEquivFun.eff {α β : U} (E : α ⟷ β) (γ : U) (F : β ⟷ γ) : (compEquivFun E γ) F = compEquiv E F :=
+  by apply HasInternalFunctors.fromBundled.eff
+  @[simp] theorem compEquivFun.to.effEff  {α β : U} (E : α ⟷ β) (γ : U) (F : β ⟷ γ) (a : α) :
+    HasInternalEquivalences.to  ((compEquivFun E γ) F) a = HasInternalEquivalences.to  F (HasInternalEquivalences.to  E a) :=
+  by simp
+  @[simp] theorem compEquivFun.inv.effEff {α β : U} (E : α ⟷ β) (γ : U) (F : β ⟷ γ) (c : γ) :
+    HasInternalEquivalences.inv ((compEquivFun E γ) F) c = HasInternalEquivalences.inv E (HasInternalEquivalences.inv F c) :=
+  by simp
+
+  def compEquivFunFun' (α β γ : U) : (α ⟷ β) ⟶' (β ⟷ γ) ⟶ (α ⟷ γ) := BundledFunctor.mkFun (h.compEquivFunIsFun α β γ)
+  def compEquivFunFun  (α β γ : U) : (α ⟷ β) ⟶  (β ⟷ γ) ⟶ (α ⟷ γ) := HasInternalFunctors.fromBundled (compEquivFunFun' α β γ)
+  
+  @[simp] theorem compEquivFunFun.eff (α β γ : U) (E : α ⟷ β) : (compEquivFunFun α β γ) E = compEquivFun E γ :=
+  by apply HasInternalFunctors.fromBundled.eff
+  @[simp] theorem compEquivFunFun.effEff (α β γ : U) (E : α ⟷ β) (F : β ⟷ γ) : ((compEquivFunFun α β γ) E) F = compEquiv E F :=
+  by simp
+  @[simp] theorem compEquivFunFun.to.effEffEff  (α β γ : U) (E : α ⟷ β) (F : β ⟷ γ) (a : α) :
+    HasInternalEquivalences.to  (((compEquivFunFun α β γ) E) F) a = HasInternalEquivalences.to  F (HasInternalEquivalences.to  E a) := by simp
+  @[simp] theorem compEquivFunFun.inv.effEffEff (α β γ : U) (E : α ⟷ β) (F : β ⟷ γ) (c : γ) :
+    HasInternalEquivalences.inv (((compEquivFunFun α β γ) E) F) c = HasInternalEquivalences.inv E (HasInternalEquivalences.inv F c) := by simp
+
+  def invEquiv' {α β : U} (E : α ⟷' β) : β ⟷' α := HasInvEquiv.invEquiv' E
+  def invEquiv  {α β : U} (E : α ⟷  β) : β ⟷  α :=
+  HasInternalEquivalences.fromBundled (invEquiv' (HasInternalEquivalences.toBundled E))
+
+  @[simp] theorem invEquiv.to.eff  {α β : U} (E : α ⟷ β) (b : β) : HasInternalEquivalences.to  (invEquiv E) b = HasInternalEquivalences.inv E b :=
+  by apply HasInternalEquivalences.fromBundled.to.eff
+  @[simp] theorem invEquiv.inv.eff {α β : U} (E : α ⟷ β) (a : α) : HasInternalEquivalences.inv (invEquiv E) a = HasInternalEquivalences.to  E a :=
+  by apply HasInternalEquivalences.fromBundled.inv.eff
+
+  def invEquivFun' (α β : U) : (α ⟷ β) ⟶' (β ⟷ α) := BundledFunctor.mkFun (h.invEquivIsFun α β)
+  def invEquivFun  (α β : U) : (α ⟷ β) ⟶  (β ⟷ α) := HasInternalFunctors.fromBundled (invEquivFun' α β)
+
+  @[simp] theorem invEquivFun.eff (α β : U) (E : α ⟷ β) : (invEquivFun α β) E = invEquiv E :=
+  by apply HasInternalFunctors.fromBundled.eff
+  @[simp] theorem invEquivFun.to.effEff  (α β : U) (E : α ⟷ β) (b : β) :
+    HasInternalEquivalences.to  ((invEquivFun α β) E) b = HasInternalEquivalences.inv E b := by simp
+  @[simp] theorem invEquivFun.inv.effEff (α β : U) (E : α ⟷ β) (a : α) :
+    HasInternalEquivalences.inv ((invEquivFun α β) E) a = HasInternalEquivalences.to  E a := by simp
+
+  def invEquivEquiv' (α β : U) : (α ⟷ β) ⟷' (β ⟷ α) := BundledEquivalence.mkEquiv (h.invEquivIsEquiv α β)
+  def invEquivEquiv  (α β : U) : (α ⟷ β) ⟷  (β ⟷ α) := HasInternalEquivalences.fromBundled (invEquivEquiv' α β)
+
+  @[simp] theorem invEquivEquiv.to.eff  (α β : U) (E : α ⟷ β) : HasInternalEquivalences.to  (invEquivEquiv α β) E = invEquiv E :=
+  by apply HasInternalEquivalences.fromBundled.to.eff
+  @[simp] theorem invEquivEquiv.inv.eff (α β : U) (E : β ⟷ α) : HasInternalEquivalences.inv (invEquivEquiv α β) E = invEquiv E :=
+  by apply HasInternalEquivalences.fromBundled.inv.eff
+  @[simp] theorem invEquivEquiv.to.to.effEff   (α β : U) (E : α ⟷ β) (b : β) :
+    HasInternalEquivalences.to  (HasInternalEquivalences.to  (invEquivEquiv α β) E) b = HasInternalEquivalences.inv E b := by simp
+  @[simp] theorem invEquivEquiv.to.inv.effEff  (α β : U) (E : α ⟷ β) (a : α) :
+    HasInternalEquivalences.inv (HasInternalEquivalences.to  (invEquivEquiv α β) E) a = HasInternalEquivalences.to  E a := by simp
+  @[simp] theorem invEquivEquiv.inv.to.effEff  (α β : U) (E : β ⟷ α) (a : α) :
+    HasInternalEquivalences.to  (HasInternalEquivalences.inv (invEquivEquiv α β) E) a = HasInternalEquivalences.inv E a := by simp
+  @[simp] theorem invEquivEquiv.inv.inv.effEff (α β : U) (E : β ⟷ α) (b : β) :
+    HasInternalEquivalences.inv (HasInternalEquivalences.inv (invEquivEquiv α β) E) b = HasInternalEquivalences.to  E b := by simp
+
+end HasEquivOp
+
+
+
+def ExternalProduct {U : Universe.{u}} {V : Universe.{v}} (α : U) (β : V) := PProd ⌈α⌉ ⌈β⌉
+
+namespace ExternalProduct
+
+  infixr:35 " ⊓' " => ExternalProduct
+
+end ExternalProduct
+
+class HasInternalProducts (U : Universe.{u}) [h : HasExternalFunctors U U] where
+(Prod                                                   : U → U → U)
+(prodEquiv        (α β : U)                             : ⌈Prod α β⌉ ≃ (α ⊓' β))
+(prodIntroIsFun   {α β ω : U} (F : ω ⟶' α) (G : ω ⟶' β) : h.IsFun (λ a : ω => (prodEquiv α β).invFun ⟨F a, G a⟩))
+(prodElimFstIsFun (α β : U)                             : h.IsFun (λ P : Prod α β => ((prodEquiv α β).toFun P).fst))
+(prodElimSndIsFun (α β : U)                             : h.IsFun (λ P : Prod α β => ((prodEquiv α β).toFun P).snd))
+
+namespace HasInternalProducts
+
+  infixr:35 " ⊓ " => HasInternalProducts.Prod
+
+end HasInternalProducts
+
+-- TODO: Add a type class that says that the combination of intro and elim are equivalences (when the other side is fixed).
+-- Prove that this is an equivalence between U and U ⨯ U.
+
+
+
+class HasEmptyType (U : Universe.{u}) [h : HasExternalFunctors U U] where
+(Empty                  : U)
+(emptyIsEmpty           : ⌈Empty⌉ → False)
+(emptyElimIsFun (α : U) : h.IsFun (λ e : Empty => @False.elim ⌈α⌉ (emptyIsEmpty e)))
+
+namespace HasEmptyType
+
+  variable {U : Universe}
+  
+  def emptyElimFun' [HasExternalFunctors U U] [h : HasEmptyType U] (α : U) : h.Empty ⟶' α :=
+  BundledFunctor.mkFun (h.emptyElimIsFun α)
+  def emptyElimFun  [HasInternalFunctors U]   [h : HasEmptyType U] (α : U) : h.Empty ⟶  α :=
+  HasInternalFunctors.fromBundled (emptyElimFun' α)
+
+  def Not [HasInternalFunctors U] [h : HasEmptyType U] (α : U) := α ⟶ h.Empty
+
+end HasEmptyType
+
+-- TODO: Can we prove `α ⟶ Not α ⟶ β`?
+
+class HasClassicalLogic (U : Universe.{u}) [HasInternalFunctors U] [h : HasEmptyType U] where
+(byContradiction (α : U) : HasEmptyType.Not (HasEmptyType.Not α) ⟶ α)
+
+
+
+class HasUnitType (U : Universe.{u}) [h : HasExternalFunctors U U] where
+(Unit                   : U)
+(unit                   : Unit)
+(unitIntroIsFun (α : U) : h.IsFun (λ a : α => unit))
+
+namespace HasUnitType
+
+  variable {U : Universe}
+  
+  def unitIntroFun' [HasExternalFunctors U U] [h : HasUnitType U] (α : U) : α ⟶' h.Unit :=
+  BundledFunctor.mkFun (h.unitIntroIsFun α)
+  def unitIntroFun  [HasInternalFunctors U]   [h : HasUnitType U] (α : U) : α ⟶  h.Unit :=
+  HasInternalFunctors.fromBundled (unitIntroFun' α)
+
+  @[simp] theorem unitIntroFun.eff [HasInternalFunctors U] [h : HasUnitType U] (α : U) (a : α) :
+    (unitIntroFun α) a = h.unit :=
+  by apply HasInternalFunctors.fromBundled.eff
+
+end HasUnitType
+
+
+
+-- TODO: Derive some logic and especially the arrow/product laws.
 
 
 
@@ -378,24 +882,39 @@ namespace GeneralizedRelation
 
     variable (R : GeneralizedRelation α V)
 
-    class HasRefl  where
-    (refl  (a     : α) : R a a)
+    class HasRefl where
+    (refl (a : α) : R a a)
 
     variable [HasInternalFunctors V]
-
-    class HasSymm  where
-    (symm  {a b   : α} : R a b ⟶ R b a)
 
     class HasTrans where
     (trans {a b c : α} : R a b ⟶ R b c ⟶ R a c)
 
-    class IsPreorder    extends HasRefl R, HasTrans R
+    class IsPreorder extends HasRefl R, HasTrans R
+
+    variable [HasInternalEquivalences V]
+
+    class HasSymm where
+    (symm {a b : α} : R a b ⟷ R b a)
+
     class IsEquivalence extends IsPreorder R, HasSymm R
   
   end Properties
 
-  def HasSymm.symm'   {R : GeneralizedRelation α V} [HasInternalFunctors V] [h : HasSymm  R] {a b   : α} (f : R a b) : R b a := h.symm f
-  def HasTrans.trans' {R : GeneralizedRelation α V} [HasInternalFunctors V] [h : HasTrans R] {a b c : α} (f : R a b) (g : R b c) : R a c := h.trans f g
+  def HasTrans.revTrans {R : GeneralizedRelation α V} [HasInternalFunctors V] [HasLinearFunOp V] [h : HasTrans R]
+                        {a b c : α} : R b c ⟶ R a b ⟶ R a c :=
+  HasLinearFunOp.swapFunFun h.trans
+
+  @[simp] theorem HasTrans.revTrans.eff {R : GeneralizedRelation α V} [HasInternalFunctors V] [HasLinearFunOp V] [h : HasTrans R]
+                                        {a b c : α} (g : R b c) (f : R a b) :
+    h.revTrans g f = h.trans f g :=
+  by apply HasLinearFunOp.swapFunFun.effEff
+
+  def HasTrans.trans' {R : GeneralizedRelation α V} [HasInternalFunctors V] [h : HasTrans R]
+                      {a b c : α} (f : R a b) (g : R b c) : R a c := h.trans f g
+
+  def HasSymm.symm' {R : GeneralizedRelation α V} [HasInternalFunctors V] [HasInternalEquivalences V] [h : HasSymm R]
+                    {a b : α} (f : R a b) : R b a := HasInternalEquivalences.to h.symm f
 
   -- When reasoning about instances of `R a b`, we would like to write `trans` as composition, `refl` as
   -- identity, and `symm` as inverse.
@@ -408,7 +927,7 @@ namespace GeneralizedRelation
 
     @[reducible] def ident (R : GeneralizedRelation α V) [h : HasRefl R] (a : α) : R a a := h.refl a
 
-    @[reducible] def inv {R : GeneralizedRelation α V} [HasInternalFunctors V] [h : HasSymm R] {a b : α} (f : R a b) : R b a := h.symm' f
+    @[reducible] def inv {R : GeneralizedRelation α V} [HasInternalFunctors V] [HasInternalEquivalences V] [h : HasSymm R] {a b : α} (f : R a b) : R b a := h.symm' f
     postfix:max "⁻¹" => inv
 
   end Notation
@@ -457,36 +976,40 @@ namespace GeneralizedDependentRelation
 
     variable (D : GeneralizedDependentRelation R W)
 
-    class HasDependentRefl  [h : HasRefl  R] where
-    (refl  {α     : U}                         (a : α)                 : D (h.refl α) a a)
+    class HasDependentRefl [h : HasRefl R] where
+    (refl {α : U} (a : α) : D (h.refl α) a a)
 
     def reflRel [h : HasRefl R] (α : U) : GeneralizedRelation ⌈α⌉ W := D (h.refl α)
     instance [HasRefl R] [h : HasDependentRefl D] (α : U) : HasRefl (reflRel D α) := ⟨h.refl⟩
 
     variable [HasInternalFunctors V] [HasInternalFunctors W]
 
-    class HasDependentSymm  [h : HasSymm  R] where
-    (symm  {α β   : U} {F : R α β}             {a : α} {b : β}         : D F a b ⟶ D (h.symm' F) b a)
-
     class HasDependentTrans [h : HasTrans R] where
     (trans {α β γ : U} {F : R α β} {G : R β γ} {a : α} {b : β} {c : γ} : D F a b ⟶ D G b c ⟶ D (h.trans' F G) a c)
 
-    class IsDependentPreorder    [h : IsPreorder    R] extends HasDependentRefl D, HasDependentTrans D
+    class IsDependentPreorder [h : IsPreorder R] extends HasDependentRefl D, HasDependentTrans D
+
+    variable [HasInternalEquivalences V] [HasInternalEquivalences W]
+
+    class HasDependentSymm [h : HasSymm R] where
+    (symm {α β : U} {F : R α β} {a : α} {b : β} : D F a b ⟷ D (h.symm' F) b a)
+
     class IsDependentEquivalence [h : IsEquivalence R] extends IsDependentPreorder D, HasDependentSymm D
 
   end Properties
 
-  def HasDependentSymm.symm'    {D : GeneralizedDependentRelation R W}
-                                [HasInternalFunctors V] [HasInternalFunctors W] [HasSymm  R] [h : HasDependentSymm  D]
-                                {α β : U} {F : R α β} {a : α} {b : β} (f : D F a b) :
-   D (HasSymm.symm' F) b a :=
-  h.symm f
-
-  def HasDependentTrans.trans'  {D : GeneralizedDependentRelation R W}
-                                [HasInternalFunctors V] [HasInternalFunctors W] [HasTrans R] [h : HasDependentTrans D]
-                                {α β γ : U} {F : R α β} {G : R β γ} {a : α} {b : β} {c : γ} (f : D F a b) (g : D G b c) :
+  def HasDependentTrans.trans' {D : GeneralizedDependentRelation R W}
+                               [HasInternalFunctors V] [HasInternalFunctors W] [HasTrans R] [h : HasDependentTrans D]
+                               {α β γ : U} {F : R α β} {G : R β γ} {a : α} {b : β} {c : γ} (f : D F a b) (g : D G b c) :
     D (HasTrans.trans' F G) a c :=
   h.trans f g
+
+  def HasDependentSymm.symm' {D : GeneralizedDependentRelation R W}
+                             [HasInternalFunctors V] [HasInternalFunctors W] [HasInternalEquivalences V] [HasInternalEquivalences W]
+                             [HasSymm  R] [h : HasDependentSymm  D]
+                             {α β : U} {F : R α β} {a : α} {b : β} (f : D F a b) :
+   D (HasSymm.symm' F) b a :=
+  HasInternalEquivalences.to h.symm f
 
   section Notation
 
@@ -502,9 +1025,10 @@ namespace GeneralizedDependentRelation
       D (ident R α) a a :=
     h.refl a
 
-    @[reducible] def depInv {D : GeneralizedDependentRelation R W} [HasInternalFunctors V] [HasInternalFunctors W]
-               [HasSymm R] [h : HasDependentSymm D]
-               {α β : U} {F : R α β} {a : α} {b : β} (f : D F a b) :
+    @[reducible] def depInv {D : GeneralizedDependentRelation R W}
+                            [HasInternalFunctors V] [HasInternalFunctors W] [HasInternalEquivalences V] [HasInternalEquivalences W]
+                            [HasSymm R] [h : HasDependentSymm D]
+                            {α β : U} {F : R α β} {a : α} {b : β} (f : D F a b) :
       D F⁻¹ b a :=
     h.symm' f
     --postfix:max "⁻¹" => depInv
@@ -524,19 +1048,6 @@ section AttachedRelations
 
   variable (α : Sort u) (V : Universe.{v}) [HasInternalFunctors V]
 
-  -- TODO: Remove this?
-  class HasProducts where
-  (Product : GeneralizedRelation α V)
-  [hasSymm : HasSymm Product]
-
-  namespace HasProducts
-    variable [h : HasProducts α V]
-    instance productSymm : HasSymm h.Product := h.hasSymm
-    instance hasProduct : HasProduct α α := ⟨h.Product⟩
-    instance : HasInstances (HasProduct.γ α α) := Universe.instInst V
-    instance : HasSymm (@HasProduct.Product α α (hasProduct α V)) := h.hasSymm
-  end HasProducts
-
   class HasArrows where
   (Arrow      : GeneralizedRelation α V)
   [isPreorder : IsPreorder Arrow]
@@ -548,6 +1059,8 @@ section AttachedRelations
     instance : HasInstances (HasArrow.γ α α) := Universe.instInst V
     instance : IsPreorder (@HasArrow.Arrow α α (hasArrow α V)) := h.isPreorder
   end HasArrows
+
+  variable [HasInternalEquivalences V]
 
   class HasEquivalences where
   (Equiv   : GeneralizedRelation α V)
@@ -561,6 +1074,18 @@ section AttachedRelations
     instance : IsEquivalence (@HasEquivalence.Equiv α α (hasEquivalence α V)) := h.isEquiv
   end HasEquivalences
 
+  class HasProducts where
+  (Product : GeneralizedRelation α V)
+  [hasSymm : HasSymm Product]
+
+  namespace HasProducts
+    variable [h : HasProducts α V]
+    instance productSymm : HasSymm h.Product := h.hasSymm
+    instance hasProduct : HasProduct α α := ⟨h.Product⟩
+    instance : HasInstances (HasProduct.γ α α) := Universe.instInst V
+    instance : HasSymm (@HasProduct.Product α α (hasProduct α V)) := h.hasSymm
+  end HasProducts
+
 end AttachedRelations
 
 
@@ -568,17 +1093,6 @@ end AttachedRelations
 section AttachedDependentRelations
 
   variable (U V W : Universe) [HasInternalFunctors V] [HasInternalFunctors W]
-
-  class HasDependentProducts [h : HasProducts ⌈U⌉ V] where
-  (Product : GeneralizedDependentRelation h.Product W)
-  [hasSymm : HasDependentSymm Product]
-
-  namespace HasDependentProducts
-    variable [HasProducts ⌈U⌉ V] [h : HasDependentProducts U V W]
-    instance productSymm : HasDependentSymm h.Product := h.hasSymm
-    notation:35 a:36 " ⊓[" P:0 "] " b:36 => HasDependentProducts.Product P a b
-    notation:35 a:36 " ⊓[" P:0 "," V':0 "," W':0 "] " b:36 => HasDependentProducts.Product (V := V') (W := W') P a b
-  end HasDependentProducts
 
   class HasDependentArrows [h : HasArrows ⌈U⌉ V] where
   (Arrow      : GeneralizedDependentRelation h.Arrow W)
@@ -591,6 +1105,8 @@ section AttachedDependentRelations
     notation:20 a:21 " ⇝[" F:0 "," V':0 "," W':0 "] " b:21 => HasDependentArrows.Arrow (V := V') (W := W') F a b
   end HasDependentArrows
 
+  variable [HasInternalEquivalences V] [HasInternalEquivalences W]
+
   class HasDependentEquivalences [h : HasEquivalences ⌈U⌉ V] where
   (Equiv   : GeneralizedDependentRelation h.Equiv W)
   [isEquiv : IsDependentEquivalence Equiv]
@@ -602,6 +1118,17 @@ section AttachedDependentRelations
     notation:25 a:26 " ≃[" F:0 "," V':0 "," W':0 "] " b:26 => HasDependentEquivalences.Equiv (V := V') (W := W') F a b
   end HasDependentEquivalences
 
+  class HasDependentProducts [h : HasProducts ⌈U⌉ V] where
+  (Product : GeneralizedDependentRelation h.Product W)
+  [hasSymm : HasDependentSymm Product]
+
+  namespace HasDependentProducts
+    variable [HasProducts ⌈U⌉ V] [h : HasDependentProducts U V W]
+    instance productSymm : HasDependentSymm h.Product := h.hasSymm
+    notation:35 a:36 " ⧆[" P:0 "] " b:36 => HasDependentProducts.Product P a b
+    notation:35 a:36 " ⧆[" P:0 "," V':0 "," W':0 "] " b:36 => HasDependentProducts.Product (V := V') (W := W') P a b
+  end HasDependentProducts
+
 end AttachedDependentRelations
 
 
@@ -610,62 +1137,11 @@ end AttachedDependentRelations
 -- frequently be an equality or at least a setoid equivalence, we need to prepare for the most generic
 -- case where equivalences are arbitrary objects. Since we then need to define a relation into the type
 -- of equivalences, we need to bundle equivalences with their equivalences.
---
--- TODO: describe arrows
-
-class HasInstanceArrows (U : Universe.{u}) where
-(arrowUniverse           : Universe.{v})
-[arrowHasFun             : HasInternalFunctors arrowUniverse]
-(Arrow (α : U)           : GeneralizedRelation ⌈α⌉ arrowUniverse)
-[arrowIsPreorder (α : U) : IsPreorder (Arrow α)]
-
-namespace HasInstanceArrows
-
-  variable (U : Universe) [h : HasInstanceArrows U]
-
-  instance hasFun : HasInternalFunctors h.arrowUniverse := h.arrowHasFun
-
-  instance arrowPreorder (α : U) : IsPreorder (h.Arrow α) := h.arrowIsPreorder α
-
-  instance hasArrows (α : U) : HasArrows ⌈α⌉ h.arrowUniverse := ⟨h.Arrow α⟩
-  @[reducible] def InstArrowType (α : U) := ⌈α⌉ (⇝) ⌈α⌉
-  instance (α : U) : HasInstances (InstArrowType U α) := Universe.instInst h.arrowUniverse
-
-end HasInstanceArrows
-
-class HasArrowCongrArg (U V : Universe) [HasExternalFunctors U V]
-                       [hU : HasInstanceArrows U] [hV : HasInstanceArrows V]
-                       [HasExternalFunctors hU.arrowUniverse hV.arrowUniverse] where
-(arrowCongrArg {α : U} {β : V} (F : α ⟶' β) {a b : α} : (a ⇝ b) ⟶' (F a ⇝ F b))
-
-class HasFunctorialArrows (U : Universe) [HasInternalFunctors U] extends HasInstanceArrows U where
-(arrowCongr {α β : U} {F G : α ⟶ β} {a b : α} : (F ⇝ G) ⟶ (a ⇝ b) ⟶ (F a ⇝ G b))
-
-namespace HasFunctorialArrows
-
-  variable (U : Universe) [HasInternalFunctors U] [h : HasFunctorialArrows U]
-
-  def arrow_congr   {α β : U} {F G : α ⟶ β} {a b : α} : (F ⇝ G) ⟶ (a ⇝ b) ⟶ (F a ⇝ G b) := h.arrowCongr
-  def arrow_congr'  {α β : U} {F G : α ⟶ β} {a b : α} : (F ⇝ G) → ((a ⇝ b) ⟶ (F a ⇝ G b)) := HasInternalFunctors.funCoe (arrow_congr U)
-  def arrow_congr'' {α β : U} {F G : α ⟶ β} {a b : α} : (F ⇝ G) → (a ⇝ b) → (F a ⇝ G b) := λ f => HasInternalFunctors.funCoe (arrow_congr' U f)
-
-  def arrow_congrArg    {α β : U} (F : α ⟶  β) {a b : α} : (a ⇝ b) ⟶ (F a ⇝ F b) := (arrow_congr' U) (HasRefl.refl F)
-  def arrow_congrArg'   {α β : U} (F : α ⟶  β) {a b : α} : (a ⇝ b) → (F a ⇝ F b) := HasInternalFunctors.funCoe (arrow_congrArg U F)
-  def arrow_congrArg''  {α β : U} (F : α ⟶' β) {a b : α} : (a ⇝ b) ⟶ (F a ⇝ F b) := HasInternalFunctors.fromBundled.coe F ▸ arrow_congrArg U (HasInternalFunctors.fromBundled F)
-  def arrow_congrArg''' {α β : U} (F : α ⟶' β) {a b : α} : (a ⇝ b) → (F a ⇝ F b) := HasInternalFunctors.funCoe (arrow_congrArg'' U F)
-
-  def arrow_congrFun [HasLinearFunOp h.arrowUniverse] {α β : U} {F G : α ⟶ β} (a : α) : (F ⇝ G) ⟶ (F a ⇝ G a) :=
-  HasLinearFunOp.appFun (HasRefl.refl a) (F a ⇝ G a) ⊙ arrow_congr U
-  def arrow_congrFun' {α β : U} {F G : α ⟶ β} (a : α) : (F ⇝ G) → (F a ⇝ G a) :=
-  λ f => arrow_congr'' U f (HasRefl.refl a)
-
-  instance toHasArrowCongrArg : HasArrowCongrArg U U := ⟨λ F => HasInternalFunctors.toBundled (arrow_congrArg'' U F)⟩
-
-end HasFunctorialArrows
 
 class HasInstanceEquivalences (U : Universe.{u}) where
 (equivUniverse              : Universe.{v})
-[equivHasFun                : HasInternalFunctors equivUniverse]
+[equivHasFunOp              : HasFunOp equivUniverse]
+[equivHasEquiv              : HasInternalEquivalences equivUniverse]
 (Equiv (α : U)              : GeneralizedRelation ⌈α⌉ equivUniverse)
 [equivIsEquivalence (α : U) : IsEquivalence (Equiv α)]
 
@@ -673,19 +1149,14 @@ namespace HasInstanceEquivalences
 
   variable (U : Universe) [h : HasInstanceEquivalences U]
 
-  instance hasFun : HasInternalFunctors h.equivUniverse := h.equivHasFun
+  instance hasFunOp : HasFunOp                h.equivUniverse := h.equivHasFunOp
+  instance hasEquiv : HasInternalEquivalences h.equivUniverse := h.equivHasEquiv
 
   instance equivEquivalence (α : U) : IsEquivalence (h.Equiv α) := h.equivIsEquivalence α
 
   instance hasEquivalences (α : U) : HasEquivalences ⌈α⌉ h.equivUniverse := ⟨h.Equiv α⟩
   @[reducible] def InstEquivType (α : U) := ⌈α⌉ (≃) ⌈α⌉
   instance (α : U) : HasInstances (InstEquivType U α) := Universe.instInst h.equivUniverse
-
-  def toHasInstanceArrows : HasInstanceArrows U :=
-  { arrowUniverse   := h.equivUniverse,
-    arrowHasFun     := h.equivHasFun,
-    Arrow           := h.Equiv,
-    arrowIsPreorder := λ α => (h.equivIsEquivalence α).toIsPreorder }
 
 end HasInstanceEquivalences
 
@@ -694,34 +1165,53 @@ class HasEquivCongrArg (U V : Universe) [HasExternalFunctors U V]
                        [HasExternalFunctors hU.equivUniverse hV.equivUniverse] where
 (equivCongrArg {α : U} {β : V} (F : α ⟶' β) {a b : α} : a ≃ b ⟶' F a ≃ F b)
 
-class HasFunctorialEquivalences (U : Universe) [HasInternalFunctors U] extends HasInstanceEquivalences U where
-(equivCongr {α β : U} {F G : α ⟶ β} {a b : α} : F ≃ G ⟶ a ≃ b ⟶ F a ≃ G b)
+namespace HasEquivCongrArg
 
-namespace HasFunctorialEquivalences
+  variable (U : Universe) [HasInternalFunctors U] [HasInstanceEquivalences U] [h : HasEquivCongrArg U U]
 
-  variable (U : Universe) [HasInternalFunctors U] [h : HasFunctorialEquivalences U]
+  def equiv_congrArg' {α β : U} (F : α ⟶' β) {a b : α} : a ≃ b ⟶' F a ≃ F b := h.equivCongrArg F
+  def equiv_congrArg  {α β : U} (F : α ⟶  β) {a b : α} : a ≃ b ⟶  F a ≃ F b := HasInternalFunctors.fromBundled (equiv_congrArg' U (HasInternalFunctors.toBundled F))
 
-  def toHasFunctorialArrows : HasFunctorialArrows U :=
-  { toHasInstanceArrows := HasInstanceEquivalences.toHasInstanceArrows U,
-    arrowCongr          := h.equivCongr }
+end HasEquivCongrArg
 
-  def equiv_congr   {α β : U} {F G : α ⟶ β} {a b : α} : F ≃ G ⟶ a ≃ b ⟶ F a ≃ G b := h.equivCongr
-  def equiv_congr'  {α β : U} {F G : α ⟶ β} {a b : α} : F ≃ G → (a ≃ b ⟶ F a ≃ G b) := HasInternalFunctors.funCoe (equiv_congr U)
-  def equiv_congr'' {α β : U} {F G : α ⟶ β} {a b : α} : F ≃ G → a ≃ b → F a ≃ G b := λ e => HasInternalFunctors.funCoe (equiv_congr' U e)
+class HasEquivCongrFun (U : Universe) [HasInternalFunctors U] [HasInstanceEquivalences U] where
+(equivCongrFun {α β : U} {F G : α ⟶ β} (a : α) : F ≃ G ⟶' F a ≃ G a)
 
-  def equiv_congrArg    {α β : U} (F : α ⟶  β) {a b : α} : a ≃ b ⟶ F a ≃ F b := (equiv_congr' U) (HasRefl.refl F)
-  def equiv_congrArg'   {α β : U} (F : α ⟶  β) {a b : α} : a ≃ b → F a ≃ F b := HasInternalFunctors.funCoe (equiv_congrArg U F)
-  def equiv_congrArg''  {α β : U} (F : α ⟶' β) {a b : α} : a ≃ b ⟶ F a ≃ F b := HasInternalFunctors.fromBundled.coe F ▸ equiv_congrArg U (HasInternalFunctors.fromBundled F)
-  def equiv_congrArg''' {α β : U} (F : α ⟶' β) {a b : α} : a ≃ b → F a ≃ F b := HasInternalFunctors.funCoe (equiv_congrArg'' U F)
+namespace HasEquivCongrFun
 
-  def equiv_congrFun [HasLinearFunOp h.equivUniverse] {α β : U} {F G : α ⟶ β} (a : α) : F ≃ G ⟶ F a ≃ G a :=
-  HasLinearFunOp.appFun (HasRefl.refl a) (F a ≃ G a) ⊙ equiv_congr U
-  def equiv_congrFun' {α β : U} {F G : α ⟶ β} (a : α) : F ≃ G → F a ≃ G a :=
-  λ e => equiv_congr'' U e (HasRefl.refl a)
+  variable (U : Universe) [HasInternalFunctors U] [HasInstanceEquivalences U] [h : HasEquivCongrFun U]
 
-  instance toHasEquivCongrArg : HasEquivCongrArg U U := ⟨λ F => HasInternalFunctors.toBundled (equiv_congrArg'' U F)⟩
+  def equiv_congrFun' {α β : U} {F G : α ⟶ β} (a : α) : F ≃ G ⟶' F a ≃ G a := h.equivCongrFun a
+  def equiv_congrFun  {α β : U} {F G : α ⟶ β} (a : α) : F ≃ G ⟶  F a ≃ G a := HasInternalFunctors.fromBundled (equiv_congrFun' U a)
 
-end HasFunctorialEquivalences
+end HasEquivCongrFun
+
+class HasEquivCongr (U : Universe) [HasInternalFunctors U] [HasInstanceEquivalences U] extends HasEquivCongrArg U U, HasEquivCongrFun U
+
+namespace HasEquivCongr
+
+  variable (U : Universe) [HasInternalFunctors U] [HasInstanceEquivalences U] [HasEquivCongr U]
+
+  def equiv_congr  {α β : U} {F G : α ⟶ β} {a b : α} : F ≃ G ⟶ a ≃ b ⟶ F a ≃ G b :=
+  HasLinearFunOp.swapFunFun (HasTrans.trans    ⊙ HasEquivCongrArg.equiv_congrArg U F) ⊙ HasEquivCongrFun.equiv_congrFun U b
+
+  def equiv_congr' {α β : U} {F G : α ⟶ β} {a b : α} : F ≃ G ⟶ a ≃ b ⟶ F a ≃ G b :=
+  HasLinearFunOp.swapFunFun (HasTrans.revTrans ⊙ HasEquivCongrArg.equiv_congrArg U G) ⊙ HasEquivCongrFun.equiv_congrFun U a
+
+end HasEquivCongr
+
+class HasNaturalEquivalences (U : Universe) [HasInternalFunctors U] extends HasInstanceEquivalences U, HasEquivCongr U where
+[equivHasInstEquivs                      : HasInstanceEquivalences equivUniverse]
+(isNat {α β : U} (F G : α ⟶ β) (a b : α) : HasEquivCongr.equiv_congr  U (F := F) (G := G) (a := a) (b := b) ≃
+                                           HasEquivCongr.equiv_congr' U (F := F) (G := G) (a := a) (b := b))
+
+namespace HasNaturalEquivalences
+
+  variable (U : Universe) [HasInternalFunctors U] [h : HasNaturalEquivalences U]
+
+  instance equivEquivs : HasInstanceEquivalences h.equivUniverse := h.equivHasInstEquivs
+
+end HasNaturalEquivalences
 
 
 
@@ -753,31 +1243,70 @@ end HasFunctorialEquivalences
 
 section Morphisms
 
-  variable {α : Sort u} {V : Universe.{v}} [HasInternalFunctors V] [HasInstanceArrows.{v, w} V]
+  variable {α : Sort u} {V : Universe.{v}} [HasInternalFunctors V] [HasInstanceEquivalences.{v, w} V]
            (R : GeneralizedRelation α V)
 
-  class IsCompositionRelation [HasTrans      R]                                 : Sort (max 1 u v w) where
-  (assocLR {a b c d : α} (f : R a b) (g : R b c) (h : R c d) : (h • g) • f ⇝ h • (g • f))
-  (assocRL {a b c d : α} (f : R a b) (g : R b c) (h : R c d) : h • (g • f) ⇝ (h • g) • f)
+  variable [HasLinearFunOp V] [HasTrans R]
 
-  class IsMorphismRelation    [IsPreorder    R] extends IsCompositionRelation R : Sort (max 1 u v w) where
-  (leftId  {a b : α} (f : R a b) : ident R b • f ⇝ f)
-  (rightId {a b : α} (f : R a b) : f • ident R a ⇝ f)
+  @[reducible] def compCompRight (a b c d : α) : R a b ⟶ R b c ⟶ R c d ⟶ R a d :=
+  HasLinearFunOp.revCompFunFun (R b c) HasTrans.trans ⊙ HasTrans.trans
+  @[reducible] def compCompLeft  (a b c d : α) : R a b ⟶ R b c ⟶ R c d ⟶ R a d :=
+  HasLinearFunOp.swapFunFun (HasLinearFunOp.compFunFunFun (R c d) (R b d) (R a d) ⊙ HasTrans.trans) ⊙ HasTrans.trans
 
-  class IsIsomorphismRelation [IsEquivalence R] extends IsMorphismRelation    R : Sort (max 1 u v w) where
-  (leftInv  {a b   : α} (f : R a b)             : f⁻¹ • f       ⇝ ident R a)
-  (rightInv {a b   : α} (f : R a b)             : f • f⁻¹       ⇝ ident R b)
-  (invInv   {a b   : α} (f : R a b)             : (f⁻¹)⁻¹       ⇝ f)
-  (compInv  {a b c : α} (f : R a b) (g : R b c) : (g • f)⁻¹     ⇝ f⁻¹ • g⁻¹)
-  (idInv    (a     : α)                         : (ident R a)⁻¹ ⇝ ident R a)
+  theorem compCompRight.eff [HasEquivCongrFun V] {a b c d : α} (f : R a b) (g : R b c) (h : R c d) :
+    (compCompRight R a b c d) f g h = h • (g • f) :=
+  by simp; rfl
+  theorem compCompLeft.eff  [HasEquivCongrFun V] {a b c d : α} (f : R a b) (g : R b c) (h : R c d) :
+    (compCompLeft  R a b c d) f g h = (h • g) • f :=
+  by simp; rfl
+
+  class IsCompositionRelation                                 : Sort (max 1 u v w) where
+  (assoc {a b c d : α} : compCompRight R a b c d ≃ compCompLeft R a b c d)
+
+  variable [HasRefl R]
+
+  @[reducible] def leftMulId  (a b : α) : R a b ⟶ R a b := HasTrans.revTrans ⟮ident R b⟯
+  @[reducible] def rightMulId (a b : α) : R a b ⟶ R a b := HasTrans.trans    ⟮ident R a⟯
+
+  theorem leftMulId.eff  [HasEquivCongrFun V] {a b : α} (f : R a b) : (leftMulId  R a b) f = ident R b • f :=
+  by simp; rfl
+  theorem rightMulId.eff [HasEquivCongrFun V] {a b : α} (f : R a b) : (rightMulId R a b) f = f • ident R a :=
+  rfl
+
+  class IsMorphismRelation    extends IsCompositionRelation R : Sort (max 1 u v w) where
+  (leftId  {a b : α} : leftMulId  R a b ≃ HasLinearFunOp.idFun (R a b))
+  (rightId {a b : α} : rightMulId R a b ≃ HasLinearFunOp.idFun (R a b))
+
+  variable [HasSubLinearFunOp V] [HasNonLinearFunOp V] [HasInternalEquivalences V] [HasSymm R]
+
+  @[reducible] def leftMulInv  (a b : α) : R a b ⟶ R a a :=
+  HasNonLinearFunOp.dupFun (HasTrans.revTrans ⊙ HasInternalEquivalences.toFun HasSymm.symm)
+  @[reducible] def rightMulInv (a b : α) : R a b ⟶ R b b :=
+  HasNonLinearFunOp.dupFun (HasTrans.trans    ⊙ HasInternalEquivalences.toFun HasSymm.symm)
+
+  theorem leftMulInv.eff  [HasEquivCongrFun V] {a b : α} (f : R a b) : (leftMulInv  R a b) f = f⁻¹ • f :=
+  by simp; rfl
+  theorem rightMulInv.eff [HasEquivCongrFun V] {a b : α} (f : R a b) : (rightMulInv R a b) f = f • f⁻¹ :=
+  by simp; rfl
+
+  class IsIsomorphismRelation extends IsMorphismRelation    R : Sort (max 1 u v w) where
+  (leftInv  {a b : α} : leftMulInv  R a b ≃ HasSubLinearFunOp.constFun (R a b) (ident R a))
+  (rightInv {a b : α} : rightMulInv R a b ≃ HasSubLinearFunOp.constFun (R a b) (ident R b))
+
+  -- TODO: convert to lemmas?
+  --(invInv   {a b   : α} (f : R a b)             : (f⁻¹)⁻¹       ≃ f)
+  --(compInv  {a b c : α} (f : R a b) (g : R b c) : (g • f)⁻¹     ≃ f⁻¹ • g⁻¹)
+  --(idInv    (a     : α)                         : (ident R a)⁻¹ ≃ ident R a)
 
 end Morphisms
 
 
 
+-- TODO: Rephrase trans and symm as functor composition.
+
 section Functors
 
-  variable {α : Sort u} {V W : Universe} [HasInstanceArrows W] [HasExternalFunctors V W]
+  variable {α : Sort u} {V W : Universe} [HasInstanceEquivalences W] [HasExternalFunctors V W]
            (R : GeneralizedRelation α V) (S : GeneralizedRelation α W)
 
   def BaseFunctor := ∀ {a b}, R a b ⟶' S a b
@@ -785,17 +1314,20 @@ section Functors
   variable (F : BaseFunctor R S)
 
   class IsReflFunctor  [hR : HasRefl  R] [hS : HasRefl  S] where
-  (respectsRefl  (a     : α)                         : F (hR.refl   a)   ⇝ hS.refl   a)
+  (respectsRefl  (a     : α)                         : F (hR.refl   a)   ≃ hS.refl   a)
 
   variable [HasInternalFunctors V] [HasInternalFunctors W]
 
-  class IsSymmFunctor  [hR : HasSymm  R] [hS : HasSymm  S] where
-  (respectsSymm  {a b   : α} (f : R a b)             : F (hR.symm'  f)   ⇝ hS.symm'  (F f))
-
   class IsTransFunctor [hR : HasTrans R] [hS : HasTrans S] where
-  (respectsTrans {a b c : α} (f : R a b) (g : R b c) : F (hR.trans' f g) ⇝ hS.trans' (F f) (F g))
+  (respectsTrans {a b c : α} (f : R a b) (g : R b c) : F (hR.trans' f g) ≃ hS.trans' (F f) (F g))
 
-  class IsPreorderFunctor    [IsPreorder    R] [IsPreorder    S] extends IsReflFunctor R S F, IsTransFunctor R S F
+  class IsPreorderFunctor [IsPreorder R] [IsPreorder S] extends IsReflFunctor R S F, IsTransFunctor R S F
+
+  variable [HasInternalEquivalences V] [HasInternalEquivalences W]
+
+  class IsSymmFunctor  [hR : HasSymm  R] [hS : HasSymm  S] where
+  (respectsSymm  {a b   : α} (f : R a b)             : F (hR.symm'  f)   ≃ hS.symm'  (F f))
+
   class IsEquivalenceFunctor [IsEquivalence R] [IsEquivalence S] extends IsPreorderFunctor R S F, IsSymmFunctor R S F
 
 end Functors
@@ -842,7 +1374,7 @@ class HasNaturalQuantification (U₁ U₂ V W : Universe) [HasExternalFunctors U
 
 section Categories
 
-  variable (M : Universe.{v}) [HasInternalFunctors M] [HasInstanceArrows.{v, w} M] (α : Sort u)
+  variable (M : Universe.{v}) [HasInternalFunctors M] [HasLinearFunOp M] [HasInstanceEquivalences.{v, w} M] (α : Sort u)
 
   class IsCategory extends HasArrows α M : Sort (max 1 u (v + 1) w) where
   [isMor : IsMorphismRelation Arrow]
@@ -854,6 +1386,8 @@ section Categories
     instance hasMor : IsMorphismRelation h.Arrow := h.isMor
 
   end IsCategory
+
+  variable [HasSubLinearFunOp M] [HasNonLinearFunOp M] [HasInternalEquivalences M]
 
   class IsGroupoid extends HasEquivalences α M : Sort (max 1 u (v + 1) w) where
   [isIso : IsIsomorphismRelation Equiv]
@@ -870,32 +1404,70 @@ end Categories
 
 
 
-class HasInstanceMorphisms (U : Universe) [HasInternalFunctors U] extends HasFunctorialArrows U where
-[arrowHasArrows     : HasInstanceArrows arrowUniverse]
-[arrowIsMor (α : U) : IsMorphismRelation (Arrow α)]
-
-namespace HasInstanceMorphisms
-
-  variable (U : Universe) [HasInternalFunctors U] [h : HasInstanceMorphisms U]
-
-  instance arrowArrows : HasInstanceArrows h.arrowUniverse := h.arrowHasArrows
-
-  instance instIsCategory (α : U) : IsCategory h.arrowUniverse ⌈α⌉ :=
-  { isMor := h.arrowIsMor α }
-
-end HasInstanceMorphisms
-
-class HasInstanceIsomorphisms (U : Universe) [HasInternalFunctors U] extends HasFunctorialEquivalences U where
-[equivHasArrows     : HasInstanceArrows equivUniverse]
+class HasInstanceIsomorphisms (U : Universe) [HasInternalFunctors U] extends HasNaturalEquivalences U where
 [equivIsIso (α : U) : IsIsomorphismRelation (Equiv α)]
 
 namespace HasInstanceIsomorphisms
 
   variable (U : Universe) [HasInternalFunctors U] [h : HasInstanceIsomorphisms U]
 
-  instance equivArrows : HasInstanceArrows h.equivUniverse := h.equivHasArrows
-
-  instance instIsCategory (α : U) : IsGroupoid h.equivUniverse ⌈α⌉ :=
+  instance typeIsGroupoid (α : U) : IsGroupoid h.equivUniverse ⌈α⌉ :=
   { isIso := h.equivIsIso α }
 
 end HasInstanceIsomorphisms
+
+
+
+def FunctorEquiv {U : Universe} [HasInternalFunctors U] [h : HasInstanceEquivalences U] [HasEquivCongrArg U U] [HasInstanceEquivalences h.equivUniverse] {α β : U} (F G : α ⟶ β) :=
+NaturalQuantification (h.Equiv α) (h.Equiv β) (HasEquivCongrArg.equivCongrArg (HasInternalFunctors.toBundled F)) (HasEquivCongrArg.equivCongrArg (HasInternalFunctors.toBundled G))
+
+class HasFunctorExtensionality (U : Universe) [HasInternalFunctors U] [h : HasInstanceEquivalences U] [HasEquivCongrArg U U] [HasInstanceEquivalences h.equivUniverse] where
+(funEquivEquiv {α β : U} {F G : α ⟶ β} : ⌈F ≃ G⌉ ≃ FunctorEquiv F G)
+
+-- TODO: This should follow from functor extensionality. Maybe because of the special role of equality in functors?
+
+--class HasLinearFunOpMorphisms (U : Universe) [HasInternalFunctors U] [HasLinearFunOp U] [HasInstanceEquivalences U] where
+--(leftId  (α β : U) : HasLinearFunOp.revCompFunFun α (HasLinearFunOp.idFun β) ≃ HasLinearFunOp.idFun (α ⟶ β))
+--(rightId (α β : U) : HasLinearFunOp.compFunFun (HasLinearFunOp.idFun α) β ≃ HasLinearFunOp.idFun (α ⟶ β))
+
+
+
+-- TODO: Move back to `Lemmas.lean`.
+-- TODO: Add equivalences.
+-- TODO: Add (iso)morphisms as an additional type class.
+
+namespace HasLinearFunOp
+
+  variable (U : Universe) [h : HasInternalFunctors U] [HasLinearFunOp U]
+
+  instance : HasRefl    h.Fun := ⟨idFun⟩
+  instance : HasTrans   h.Fun := ⟨compFunFunFun _ _ _⟩
+  instance : IsPreorder h.Fun := ⟨⟩
+
+  instance hasArrows : HasArrows ⌈U⌉ U := ⟨h.Fun⟩
+
+  @[simp] theorem transDef {α β γ : U} {F : α ⟶ β} {G : β ⟶ γ} : G • F = G ⊙ F :=
+  compFunFunFun.effEff α β γ F G
+
+  variable [hInst : HasNaturalEquivalences U] [HasLinearFunOp hInst.equivUniverse]
+
+  def DependentArrow {α β : U} (F : α ⟶ β) (a : α) (b : β) := F a ≃ b
+
+  namespace DependentArrow
+
+    def refl {α : U} (a : α) : (idFun α) a ≃ a :=
+    Eq.ndrec (motive := λ x : α => ⌈x ≃ a⌉) (ident (hInst.Equiv α) a) (Eq.symm (idFun.eff α a))
+
+    def trans {α β γ : U} {F : α ⟶ β} {G : β ⟶ γ} {a : α} {b : β} {c : γ} : F a ≃ b ⟶ G b ≃ c ⟶ (G • F) a ≃ c :=
+    let f₁ : F a ≃ b ⟶ (G • F) a ≃ G b := compFunFunFun.effEffEff α β γ F G a ▸ HasEquivCongrArg.equiv_congrArg U G;
+    HasTrans.trans ⊙ f₁ 
+
+    instance : GeneralizedDependentRelation.HasDependentRefl    (DependentArrow U) := ⟨refl  U⟩
+    instance : GeneralizedDependentRelation.HasDependentTrans   (DependentArrow U) := ⟨trans U⟩
+    instance : GeneralizedDependentRelation.IsDependentPreorder (DependentArrow U) := ⟨⟩
+  
+  end DependentArrow
+
+  instance hasDependentArrows : HasDependentArrows U U hInst.equivUniverse := ⟨DependentArrow U⟩
+
+end HasLinearFunOp
