Structure/Generic/Instances/Setoid.lean
@@ -11,27 +11,27 @@ universes u
 
 
 def BundledSetoid := Bundled Setoid
-@[reducible] def bundledSetoid : Universe := simpleBundledUniverse Setoid
+@[reducible] def setoid : Universe := simpleBundledUniverse Setoid
 
 namespace BundledSetoid
 
-  instance isSetoid (S : bundledSetoid) : Setoid ⌈S⌉ := S.inst
-  instance (S : bundledSetoid) : Setoid ⌈S⌉ := isSetoid S
+  instance isSetoid (S : setoid) : Setoid ⌈S⌉ := S.inst
+  instance (S : setoid) : Setoid ⌈S⌉ := isSetoid S
 
-  class IsFunctorial {S T : bundledSetoid} (f : S → T) : Type u where
+  class IsFunctorial {S T : setoid} (f : S → T) : Type u where
   (mapEquiv {a b : S} : a ≈ b → f a ≈ f b)
 
   instance hasFunctoriality : Bundled.HasFunctoriality Setoid Setoid := ⟨IsFunctorial⟩
 
   namespace BundledFunctor
 
-    theorem congrArg {S T : bundledSetoid} (F : S ⟶' T) {a b : S} : a ≈ b → F a ≈ F b := F.isFun.mapEquiv
+    theorem congrArg {S T : setoid} (F : S ⟶' T) {a b : S} : a ≈ b → F a ≈ F b := F.isFun.mapEquiv
 
-    def Equiv {S T : bundledSetoid} (F G : S ⟶' T) := ∀ a, F a ≈ G a
+    def Equiv {S T : setoid} (F G : S ⟶' T) := ∀ a, F a ≈ G a
 
     namespace Equiv
 
-      variable {S T : bundledSetoid}
+      variable {S T : setoid}
 
       theorem refl  (F     : S ⟶' T)                                 : Equiv F F := λ a => Setoid.refl  (F a)
       theorem symm  {F G   : S ⟶' T} (h : Equiv F G)                 : Equiv G F := λ a => Setoid.symm  (h a)
@@ -41,11 +41,11 @@ namespace BundledSetoid
 
     end Equiv
 
-    instance isSetoid (S T : bundledSetoid) : Setoid (S ⟶' T) := ⟨Equiv, Equiv.isEquivalence⟩
+    instance isSetoid (S T : setoid) : Setoid (S ⟶' T) := ⟨Equiv, Equiv.isEquivalence⟩
 
-    theorem congrFun {S T : bundledSetoid} {F G : S ⟶' T} (h : F ≈ G) (a : S) : F a ≈ G a := h a
+    theorem congrFun {S T : setoid} {F G : S ⟶' T} (h : F ≈ G) (a : S) : F a ≈ G a := h a
 
-    theorem congr {S T : bundledSetoid} {F G : S ⟶' T} {a b : S} : F ≈ G → a ≈ b → F a ≈ G b :=
+    theorem congr {S T : setoid} {F G : S ⟶' T} {a b : S} : F ≈ G → a ≈ b → F a ≈ G b :=
     λ h₁ h₂ => Setoid.trans (congrFun h₁ a) (congrArg G h₂)
 
     instance hasFunctorInstances : Bundled.HasFunctorInstances Setoid := ⟨isSetoid⟩
@@ -54,15 +54,15 @@ namespace BundledSetoid
 
   -- Although this duplicates generic proofs in `ConstructibleFunctors.lean`, we keep this version because
   -- it is much more readable and we can avoid the import.
-  instance hasIdFun    : HasIdFun    bundledSetoid                             :=
+  instance hasIdFun    : HasIdFun    setoid                             :=
   ⟨λ S           => ⟨id⟩⟩
-  instance hasConstFun : HasConstFun bundledSetoid bundledSetoid               :=
+  instance hasConstFun : HasConstFun setoid setoid               :=
   ⟨λ S {T}   c   => ⟨λ _ => Setoid.refl c⟩⟩
-  instance hasCompFun  : HasCompFun  bundledSetoid bundledSetoid bundledSetoid :=
+  instance hasCompFun  : HasCompFun  setoid setoid setoid :=
   ⟨λ {S T U} F G => ⟨BundledFunctor.congrArg G ∘ BundledFunctor.congrArg F⟩⟩
 
   -- Same.
-  instance hasFunOp : HasFunOp bundledSetoid :=
+  instance hasFunOp : HasFunOp setoid :=
   { constFunIsFun   := λ S T       => ⟨λ hc a   => hc⟩,
     appIsFun        := λ {S} a T   => ⟨λ hF     => BundledFunctor.congrFun hF a⟩,
     appFunIsFun     := λ S T       => ⟨λ ha F   => BundledFunctor.congrArg F ha⟩,
@@ -71,11 +71,16 @@ namespace BundledSetoid
     compFunIsFun    := λ {S T} F U => ⟨λ hG a   => BundledFunctor.congrFun hG (F a)⟩,
     compFunFunIsFun := λ S T U     => ⟨λ hF G a => BundledFunctor.congrArg G (BundledFunctor.congrFun hF a)⟩ }
 
-  instance hasInstanceEquivalences : HasInstanceEquivalences bundledSetoid :=
-  ⟨propUniverse, λ S => (isSetoid S).r⟩
+  instance hasInstanceEquivalences : HasInstanceEquivalences setoid :=
+  ⟨prop, λ S => (isSetoid S).r⟩
 
-  instance hasFunctorialEquivalences : HasFunctorialEquivalences bundledSetoid :=
-  { equivCongr := BundledFunctor.congr }
+  instance hasEquivCongr : HasEquivCongr setoid :=
+  { equivCongrArg := λ F => sort.toBundledFunctor (BundledFunctor.congrArg F),
+    equivCongrFun := λ a => sort.toBundledFunctor (λ h => BundledFunctor.congrFun h a) }
+
+  instance hasNaturalEquivalences : HasNaturalEquivalences setoid :=
+  { equivHasInstEquivs := unit.hasUnitInstanceEquivalences prop,
+    isNat              := λ _ _ _ _ => trivial }
 
   def eq (α : Sort u) : BundledSetoid :=
   { α    := α,
