Structure/Generic/Instances/ConstructibleFunctors.lean
@@ -1,3 +1,5 @@
+#exit
+
 import Structure.Generic.Axioms
 import Structure.Generic.DerivedFunctors
 
