Structure/Generic/Instances/DerivedUniverses.lean
@@ -1,0 +1,27 @@
+import Structure.Generic.Axioms
+
+
+
+set_option autoBoundImplicitLocal false
+--set_option pp.universes true
+
+universes u v
+
+
+
+structure UniverseProduct (U : Universe.{u}) (V : Universe.{v}) : Type (max 1 u v) where
+(α : U)
+(β : V)
+
+def functorUniverse (U : Universe.{u}) (V : Universe.{v}) [HasExternalFunctors U V] : Universe.{max 1 u v} :=
+{ α    := UniverseProduct U V,
+  inst := ⟨λ P => P.α ⟶' P.β⟩ }
+
+def equivalenceUniverse (U : Universe.{u}) (V : Universe.{v}) [HasExternalFunctors U V] [HasExternalFunctors V U]
+                                                              [HasExternalEquivalences U V] : Universe.{max 1 u v} :=
+{ α    := UniverseProduct U V,
+  inst := ⟨λ P => P.α ⟷' P.β⟩ }
+
+def productUniverse (U : Universe.{u}) (V : Universe.{v}) : Universe.{max 1 u v} :=
+{ α    := UniverseProduct U V,
+  inst := ⟨λ P => PProd ⌈P.α⌉ ⌈P.β⌉⟩ }
